theories/Symbolic/Soundness.v
@@ -45,7 +45,7 @@ From Equations Require Import
 From Katamaran Require Import
      Shallow.Executor
      Specification
-     Symbolic.Mutator
+     Symbolic.Executor
      Symbolic.Solver
      Symbolic.Worlds
      Symbolic.Propositions
@@ -60,112 +60,120 @@ Import env.notations.
 
 Module Soundness
   (Import B    : Base)
-  (Import SIG : ProgramLogicSignature B)
+  (Import SIG  : ProgramLogicSignature B)
   (Import SPEC : Specification B SIG)
   (Import SOLV : SolverKit B SIG SPEC)
   (Import SHAL : ShallowExecOn B SIG SPEC)
-  (Import SYMB : MutatorsOn B SIG SPEC SOLV).
+  (Import SYMB : SymbolicExecOn B SIG SPEC SOLV).
 
   Import ModalNotations.
   Import SymProp.
 
-  Class Approx (AT : TYPE) (A : Type) : Type :=
-    approx :
+  (* The definition of the logical relation in the paper suggest a usual
+     recursion over the structure of types. We could define a closed universe of
+     types that we can recurse over. However, that is inconvenient for multiple
+     reasons.
+
+     1. We would need a somewhat automated mapping from types to their code in
+        the universe. Doing any kinds of tricks with typeclasses to implement
+        this is very brittle. The mechanics behind canonical structures could in
+        theory (not in actuality) implement this as well, but would suffer from
+        the same brittleness.
+
+     2. Every time we define a new type (say yet another record type that holds
+        debug information) we would have to add it to the universe.
+
+     Instead of defining a closed universe of types, we leave it open (and modular)
+     and use a type class whose method calculates the relation. This still suffers
+     a bit from 1., but avoids 2..
+     *)
+  Class Refine (AT : TYPE) (A : Type) : Type :=
+    refine :
       forall (w : World) (ι : Valuation w), (* instpc (wco w) ι -> *)
         AT w -> A -> Prop.
-  Global Arguments approx {_ _ _ w} ι _ _.
+  Global Arguments refine {_ _ _ w} ι _ _.
+  (* We use the same script ℛ as in the paper. This encodes (ι,x,y) ∈ ℛ[_,_]
+     from the paper as (ℛ ι x y), i.e. the types of the relation are implicit. *)
+  Local Notation ℛ := refine.
 
-  Global Instance ApproxInst {AT A} `{instA : Inst AT A} : Approx AT A :=
+  (* This instance can be used for any (first-class) symbolic data that can be
+     instantiated with a valuation, i.e. symbolic terms, stores, heaps etc. *)
+  Global Instance RefineInst {AT A} `{instA : Inst AT A} : Refine AT A :=
     fun w ι t v =>
       v = inst t ι.
-  Global Arguments ApproxInst {_ _ _} w ι t v /.
+  Global Arguments RefineInst {_ _ _} w ι t v /.
 
-  Global Instance ApproxPath : Approx 𝕊 Prop :=
+  (* Relatedness of symbolic and shallow propositions. The driving base case! *)
+  Global Instance RefineProp : Refine 𝕊 Prop :=
     fun w ι SP P => (wsafe SP ι -> P)%type.
 
-  Global Instance ApproxBox {AT A} `{Approx AT A} : Approx (Box AT) A :=
+  Global Instance RefineBox {AT A} `{Refine AT A} : Refine (Box AT) A :=
     fun w0 ι0 a0 a =>
       forall (w1 : World) (ω01 : w0 ⊒ w1) (ι1 : Valuation w1),
         ι0 = inst (sub_acc ω01) ι1 ->
         instpc (wco w1) ι1 ->
-        approx ι1 (a0 w1 ω01) a.
+        ℛ ι1 (a0 w1 ω01) a.
 
-  Global Instance ApproxImpl {AT A BT B} `{Approx AT A, Approx BT B} : Approx (Impl AT BT) (A -> B) :=
+  Global Instance RefineImpl {AT A BT B} `{Refine AT A, Refine BT B} :
+    Refine (Impl AT BT) (A -> B) :=
     fun w ι fs fc =>
       forall (ta : AT w) (a : A),
-        approx ι ta a ->
-        approx ι (fs ta) (fc a).
+        ℛ ι ta a ->
+        ℛ ι (fs ta) (fc a).
 
-  Global Instance ApproxForall {𝑲 : Set} {AT : forall K : 𝑲, TYPE} {A : forall K : 𝑲, Type} {apxA : forall K, Approx (AT K) (A K)} :
-    Approx (@Forall 𝑲 AT) (forall K : 𝑲, A K) :=
+  Global Instance RefineForall {𝑲} {AT : forall K : 𝑲, TYPE} {A : forall K : 𝑲, Type}
+    {refA : forall K, Refine (AT K) (A K)} :
+    Refine (@Forall 𝑲 AT) (forall K : 𝑲, A K) :=
     fun w ι fs fc =>
       forall K : 𝑲,
-        approx ι (fs K) (fc K).
+        ℛ ι (fs K) (fc K).
 
-  Global Instance ApproxMut {Γ1 Γ2 AT A} `{Approx AT A} : Approx (SMut Γ1 Γ2 AT) (CMut Γ1 Γ2 A).
-  Proof.
-    unfold SMut, CMut.
-    eapply ApproxImpl.
-  Defined.
-  (* Defined. *)
-  (*   (* fun w ι ms mc => *) *)
-  (*   (*   forall POST δt ht δc hc, *) *)
-  (*   (*     δc = inst δt ι -> *) *)
-  (*   (*     hc = inst ht ι -> *) *)
-  (*   (*     smut_wp ms POST δt ht ι -> *) *)
-  (*   (*     cmut_wp mc POST δc hc. *) *)
+  (* Try to help type class resolution. :( )*)
+  Global Instance RefineHeapSpecM {Γ1 Γ2 AT A} `{Refine AT A} :
+    Refine (SHeapSpecM Γ1 Γ2 AT) (CHeapSpecM Γ1 Γ2 A) := RefineImpl.
+  Global Instance RefineTermVal {σ} : Refine (STerm σ) (Val σ) :=
+    RefineInst (AT := STerm σ).
+  Global Instance RefineStore {Δ : PCtx} :
+    Refine (SStore Δ) (CStore Δ) := RefineInst.
+  Global Instance RefineEnv {Δ : Ctx Ty} :
+    Refine (fun w => Env (Term w) Δ) (Env Val Δ) | 1 :=
+    RefineInst.
+  Global Instance RefineNamedEnv {N : Set} {Δ : NCtx N Ty} :
+    Refine (fun w => NamedEnv (Term w) Δ) (NamedEnv Val Δ) | 1 :=
+    RefineInst.
 
-  Global Instance ApproxTermVal {σ} : Approx (STerm σ) (Val σ) :=
-    ApproxInst (AT := STerm σ).
-
-  Global Instance ApproxStore {Δ : PCtx} :
-    Approx (SStore Δ) (CStore Δ) :=
-    ApproxInst.
-
-  Global Instance ApproxNamedEnv {N : Set} {Δ : NCtx N Ty} :
-    Approx (fun w => NamedEnv (Term w) Δ) (NamedEnv Val Δ) | 1 :=
-    ApproxInst.
-
-  (* Global Instance ApproxChunk : Approx Chunk SCChunk := *)
+  (* Global Instance RefineChunk : Refine Chunk SCChunk := *)
   (*   fun w ι t v => *)
   (*     v = inst t ι. *)
 
-  (* Global Instance ApproxUnit : Approx Unit unit := *)
+  (* Global Instance RefineUnit : Refine Unit unit := *)
   (*   fun w ι t v => *)
   (*     v = inst t ι. *)
 
-  Local Hint Unfold SMut : core.
-  Local Hint Unfold CMut : core.
-
-  Local Hint Unfold SMut : typeclass_instances.
-  Local Hint Unfold CMut : typeclass_instances.
-
-  Local Hint Unfold approx ApproxImpl ApproxBox ApproxInst ApproxPath (* ApproxMut  *)ApproxTermVal (* ApproxNamedEnv *) ApproxStore : core.
+  Local Hint Unfold refine RefineBox RefineProp RefineInst RefineTermVal
+    RefineStore : core.
 
   Import ModalNotations.
   Open Scope modal.
 
-  Lemma approx_four {AT A} `{Approx AT A} {w0 : World} (ι0 : Valuation w0) :
+  Lemma refine_four {AT A} `{Refine AT A} {w0 : World} (ι0 : Valuation w0) :
     forall (a0 : Box AT w0) (a : A),
-      approx ι0 a0 a ->
+      ℛ ι0 a0 a ->
       forall w1 (ω01 : w0 ⊒ w1) (ι1 : Valuation w1),
         ι0 = inst (sub_acc ω01) ι1 ->
-        approx ι1 (four a0 ω01) a.
+        ℛ ι1 (four a0 ω01) a.
   Proof.
-    unfold approx, ApproxBox.
+    unfold ℛ, RefineBox.
     intros * H0 w1 ω01 ι1 ? w2 ω12 ι2 ? Hpc2.
     apply H0; auto.
     rewrite sub_acc_trans, inst_subst.
     now subst.
   Qed.
-  Local Hint Resolve approx_four : core.
+  Local Hint Resolve refine_four : core.
 
-  Lemma approx_lift {AT A} `{InstLift AT A} {w0 : World} (ι0 : Valuation w0) (a : A) :
-    approx ι0 (lift (T := AT) a) a.
-  Proof.
-    hnf. now rewrite inst_lift.
-  Qed.
-  Local Hint Resolve approx_lift : core.
+  Lemma refine_lift {AT A} `{InstLift AT A} {w0 : World} (ι0 : Valuation w0) (a : A) :
+    ℛ ι0 (lift (T := AT) a) a.
+  Proof. hnf. now rewrite inst_lift. Qed.
 
   Ltac wsimpl :=
     repeat
@@ -187,12 +195,12 @@ Module Soundness
          ?sub_acc_trans, ?sub_acc_triangular, ?inst_triangular_right_inverse).
        (* repeat *)
        (*   match goal with *)
-       (*   | |- approx _ (@smut_angelic _ _ _ _ _) (@cmut_angelic _ _ _) => *)
-       (*     apply approx_angelic; auto *)
-       (*   | |- approx _ (smut_pure _) (cmut_pure _) => *)
-       (*     apply approx_pure; auto *)
-       (*   | |- approx _ (smut_bind _ _) (cmut_bind _ _) => *)
-       (*     apply approx_bind; auto *)
+       (*   | |- ℛ _ (@smut_angelic _ _ _ _ _) (@cmut_angelic _ _ _) => *)
+       (*     apply refine_angelic; auto *)
+       (*   | |- ℛ _ (smut_pure _) (cmut_pure _) => *)
+       (*     apply refine_pure; auto *)
+       (*   | |- ℛ _ (smut_bind _ _) (cmut_bind _ _) => *)
+       (*     apply refine_bind; auto *)
        (*   | |- forall (_ : World) (_ : Valuation _), instpc (wco _) _ -> _ => *)
        (*     let w := fresh "w" in *)
        (*     let ι := fresh "ι" in *)
@@ -200,56 +208,57 @@ Module Soundness
        (*     intros w ι Hpc *)
        (*   end). *)
 
-  Module Path.
+  Lemma refine_symprop_angelic_binary
+    {w : World} (ι : Valuation w) (Hpc : instpc (wco w) ι) :
+    ℛ ι (@angelic_binary w) (@or).
+  Proof.
+    intros PS1 PC1 HP1 PS2 PC2 HP2.
+    intros [H1|H2]; [left|right]; auto.
+  Qed.
 
-    Lemma approx_angelic_binary
-      {w : World} (ι : Valuation w) (Hpc : instpc (wco w) ι) :
-      approx ι (@angelic_binary w) (@or).
-    Proof.
-      intros PS1 PC1 HP1 PS2 PC2 HP2.
-      intros [H1|H2]; [left|right]; auto.
-    Qed.
+  Lemma refine_symprop_demonic_binary
+    {w : World} (ι : Valuation w) (Hpc : instpc (wco w) ι) :
+    ℛ ι (@demonic_binary w) (@and).
+  Proof.
+    intros PS1 PC1 HP1 PS2 PC2 HP2.
+    intros [H1 H2]; split; auto.
+  Qed.
 
-    Lemma approx_demonic_binary
-      {w : World} (ι : Valuation w) (Hpc : instpc (wco w) ι) :
-      approx ι (@demonic_binary w) (@and).
-    Proof.
-      intros PS1 PC1 HP1 PS2 PC2 HP2.
-      intros [H1 H2]; split; auto.
-    Qed.
+  Module PureSpecM.
 
-  End Path.
-
-  Module Dijk.
-
-    Lemma approx_pure {AT A} `{Approx AT A} {w : World} (ι : Valuation w) (Hpc : instpc (wco w) ι) :
-      approx ι (@SDijk.pure AT w) CDijk.pure.
+    Lemma refine_pure {AT A} `{Refine AT A} {w : World} (ι : Valuation w) (Hpc : instpc (wco w) ι) :
+      ℛ ι (@SPureSpecM.pure AT w) CPureSpecM.pure.
     Proof.
       intros t v tv.
       intros POST__s POST__c HPOST.
-      unfold SDijk.pure, CDijk.pure.
+      unfold SPureSpecM.pure, CPureSpecM.pure.
       apply HPOST; auto. cbn.
       now rewrite inst_sub_id.
     Qed.
 
-    Lemma approx_bind {AT A BT B} `{Approx AT A, Approx BT B}
+    Lemma refine_bind {AT A BT B} `{Refine AT A, Refine BT B}
           {w0 : World} (ι0 : Valuation w0) (* (Hpc0 : instpc (wco w0) ι0) *) :
-      approx ι0 (@SDijk.bind AT BT w0) (@CDijk.bind A B).
+      ℛ ι0 (@SPureSpecM.bind AT BT w0) (@CPureSpecM.bind A B).
     Proof.
-      (* cbv [approx ApproxBox ApproxImpl ApproxMut ApproxPath ApproxInst]. *)
+      (* cbv [ℛ RefineBox RefineImpl RefineMut RefineProp RefineInst]. *)
       intros ms mc Hm fs fc Hf.
       intros POST__s POST__c HPOST.
-      unfold SDijk.bind, CDijk.bind.
+      unfold SPureSpecM.bind, CPureSpecM.bind.
       apply Hm; eauto.
       intros w1 ω01 ι1 -> Hpc1.
       intros a1 a Ha.
       apply Hf; auto.
-      eapply approx_four; eauto.
+      eapply refine_four; eauto.
     Qed.
 
-    Lemma approx_angelic (x : option 𝑺) (σ : Ty) :
+    Lemma refine_error {AT A M} `{Refine AT A, Subst M, OccursCheck M}
+      {w0 : World} (ι0 : Valuation w0) (Hpc0 : instpc (wco w0) ι0) {msg : M w0} :
+      ℛ ι0 (SPureSpecM.error (A := AT) msg) CPureSpecM.error.
+    Proof. intros POST__s POST__c HPOST. auto. Qed.
+
+    Lemma refine_angelic (x : option 𝑺) (σ : Ty) :
       forall {w0 : World} (ι0 : Valuation w0) (Hpc0 : instpc (wco w0) ι0),
-        approx ι0 (@SDijk.angelic x σ w0) (@CDijk.angelic σ).
+        ℛ ι0 (@SPureSpecM.angelic x σ w0) (@CPureSpecM.angelic σ).
     Proof.
       intros w0 ι0 Hpc0.
       intros POST__s POST__c HPOST.
@@ -259,52 +268,88 @@ Module Soundness
       reflexivity.
     Qed.
 
-    Lemma approx_angelic_ctx {N : Set} {n : N -> 𝑺} {Δ : NCtx N Ty} :
+    Lemma refine_angelic_ctx {N : Set} {n : N -> 𝑺} {Δ : NCtx N Ty} :
       forall {w0 : World} (ι0 : Valuation w0) (Hpc0 : instpc (wco w0) ι0),
-        approx ι0 (@SDijk.angelic_ctx N n w0 Δ) (@CDijk.angelic_ctx N Δ).
+        ℛ ι0 (@SPureSpecM.angelic_ctx N n w0 Δ) (@CPureSpecM.angelic_ctx N Δ).
     Proof.
-      induction Δ; cbn [SDijk.angelic_ctx CDijk.angelic_ctx].
+      induction Δ; cbn [SPureSpecM.angelic_ctx CPureSpecM.angelic_ctx].
       - intros w0 ι0 Hpc0.
-        now apply approx_pure.
+        now apply refine_pure.
       - destruct b as [x σ].
         intros w0 ι0 Hpc0.
-        apply approx_bind; [|intros w1 ω01 ι1 -> Hpc1].
-        apply approx_angelic; auto.
+        apply refine_bind; [|intros w1 ω01 ι1 -> Hpc1].
+        apply refine_angelic; auto.
         intros t v ->.
-        apply approx_bind; [|intros w2 ω12 ι2 -> Hpc2].
+        apply refine_bind; [|intros w2 ω12 ι2 -> Hpc2].
         apply IHΔ; auto.
         intros ts vs ->.
-        apply approx_pure; auto.
+        apply refine_pure; auto.
         rewrite <- inst_persist.
         reflexivity.
     Qed.
 
-    Lemma approx_demonic (x : option 𝑺) (σ : Ty) :
+    Lemma refine_demonic (x : option 𝑺) (σ : Ty) :
       forall {w0 : World} (ι0 : Valuation w0) (Hpc0 : instpc (wco w0) ι0),
-        approx ι0 (@SDijk.demonic x σ w0) (@CDijk.demonic σ).
+        ℛ ι0 (@SPureSpecM.demonic x σ w0) (@CPureSpecM.demonic σ).
     Proof.
-      intros w0 ι0 Hpc0.
-      intros POST__s POST__c HPOST.
-      intros Hwp v.
-      specialize (Hwp v).
-      revert Hwp.
-      eapply HPOST. cbn. now rewrite inst_sub_wk1.
-      cbn. now rewrite inst_subst, inst_sub_wk1.
+      intros w0 ι0 Hpc0 POST__s POST__c HPOST; cbn.
+        (* x : option 𝑺 *)
+        (* σ : Ty *)
+        (* w0 : World *)
+        (* ι0 : Valuation w0 *)
+        (* Hpc0 : instpc (wco w0) ι0 *)
+        (* POST__s : □(WTerm σ -> fun Σ : World => 𝕊 Σ) w0 *)
+        (* POST__c : Val σ -> Prop *)
+        (* HPOST : ℛ ι0 POST__s POST__c *)
+        (* ============================ *)
+        (* ℛ ι0 (SPureSpecM.demonic x σ POST__s) (CPureSpecM.demonic σ POST__c) *)
+      intros Hwp v. cbn in Hwp. specialize (Hwp v). remember (fresh w0 x) as ℓ.
+        (* x : option 𝑺 *)
+        (* σ : Ty *)
+        (* w0 : World *)
+        (* ι0 : Valuation w0 *)
+        (* Hpc0 : instpc (wco w0) ι0 *)
+        (* POST__s : □(WTerm σ -> fun Σ : World => 𝕊 Σ) w0 *)
+        (* POST__c : Val σ -> Prop *)
+        (* HPOST : ℛ ι0 POST__s POST__c *)
+        (* v : Val σ *)
+        (* ℓ : 𝑺 *)
+        (* Heqℓ : ℓ = fresh w0 x *)
+        (* Hwp : wsafe (POST__s (wsnoc w0 (ℓ∷σ)) acc_snoc_right (term_var ℓ)) ι0.[ℓ∷σ ↦ v] *)
+        (* ============================ *)
+        (* POST__c v *)
+      revert Hwp. apply HPOST;
+        [ (* Boilerplate #1 *) cbn; now rewrite inst_sub_wk1
+        | (* Boilerplate #2 *) cbn; now rewrite inst_subst, inst_sub_wk1
+        |].
+        (* x : option 𝑺 *)
+        (* σ : Ty *)
+        (* w0 : World *)
+        (* ι0 : Valuation w0 *)
+        (* Hpc0 : instpc (wco w0) ι0 *)
+        (* POST__s : □(WTerm σ -> fun Σ : World => 𝕊 Σ) w0 *)
+        (* POST__c : Val σ -> Prop *)
+        (* HPOST : ℛ ι0 POST__s POST__c *)
+        (* v : Val σ *)
+        (* ℓ : 𝑺 *)
+        (* Heqℓ : ℓ = fresh w0 x *)
+        (* ============================ *)
+        (* ℛ ι0.[ℓ∷σ ↦ v] (term_var ℓ) v *)
       reflexivity.
     Qed.
 
-    Lemma approx_demonic_ctx {N : Set} {n : N -> 𝑺} {Δ : NCtx N Ty} :
+    Lemma refine_demonic_ctx {N : Set} {n : N -> 𝑺} {Δ : NCtx N Ty} :
       forall {w0 : World} (ι0 : Valuation w0) (Hpc0 : instpc (wco w0) ι0),
-        approx ι0 (@SDijk.demonic_ctx N n w0 Δ) (@CDijk.demonic_ctx N Δ).
+        ℛ ι0 (@SPureSpecM.demonic_ctx N n w0 Δ) (@CPureSpecM.demonic_ctx N Δ).
     Proof.
       induction Δ.
       - intros w0 ι0 Hpc0.
         intros POST__s POST__c HPOST.
-        unfold SDijk.demonic_ctx, CDijk.demonic_ctx, T.
+        unfold SPureSpecM.demonic_ctx, CPureSpecM.demonic_ctx, T.
         apply HPOST; wsimpl; try reflexivity; auto.
       - destruct b as [x σ].
         intros w0 ι0 Hpc0 POST__s POST__c HPOST; cbn.
-        apply approx_demonic; auto.
+        apply refine_demonic; auto.
         intros w1 ω01 ι1 -> Hpc1.
         intros t v tv.
         apply IHΔ; auto.
@@ -316,11 +361,11 @@ Module Soundness
         reflexivity.
     Qed.
 
-    Lemma approx_assume_formulas {w0 : World} (ι0 : Valuation w0) (Hpc0 : instpc (wco w0) ι0)
+    Lemma refine_assume_formulas {w0 : World} (ι0 : Valuation w0) (Hpc0 : instpc (wco w0) ι0)
       (fmls0 : List Formula w0) (P : Prop) (Heq : instpc fmls0 ι0 <-> P) :
-      approx ι0 (@SDijk.assume_formulas w0 fmls0) (@CDijk.assume_formula P).
+      ℛ ι0 (@SPureSpecM.assume_formulas w0 fmls0) (@CPureSpecM.assume_formula P).
     Proof.
-      intros POST__s POST__c HPOST. unfold SDijk.assume_formulas.
+      intros POST__s POST__c HPOST. unfold SPureSpecM.assume_formulas.
       intros Hwp Hfmls0. apply Heq in Hfmls0.
       destruct (solver_spec fmls0) as [[w1 [ζ fmls1]] Hsolver|Hsolver].
       - specialize (Hsolver ι0 Hpc0).
@@ -337,16 +382,16 @@ Module Soundness
       - intuition.
     Qed.
 
-    Lemma approx_assume_formula {w0 : World} (ι0 : Valuation w0) (Hpc0 : instpc (wco w0) ι0)
+    Lemma refine_assume_formula {w0 : World} (ι0 : Valuation w0) (Hpc0 : instpc (wco w0) ι0)
       (fml : Formula w0) (P : Prop) (Heq : inst fml ι0 <-> P) :
-      approx ι0 (@SDijk.assume_formula w0 fml) (@CDijk.assume_formula P).
-    Proof. unfold SDijk.assume_formula. apply approx_assume_formulas; cbn; intuition. Qed.
+      ℛ ι0 (@SPureSpecM.assume_formula w0 fml) (@CPureSpecM.assume_formula P).
+    Proof. unfold SPureSpecM.assume_formula. apply refine_assume_formulas; cbn; intuition. Qed.
 
-    Lemma approx_assert_formulas {w0 : World} (ι0 : Valuation w0) (Hpc0 : instpc (wco w0) ι0)
+    Lemma refine_assert_formulas {w0 : World} (ι0 : Valuation w0) (Hpc0 : instpc (wco w0) ι0)
       (msg : AMessage w0) (fmls0 : List Formula w0) (P : Prop) (Heq : instpc fmls0 ι0 <-> P) :
-      approx ι0 (@SDijk.assert_formulas w0 msg fmls0) (@CDijk.assert_formula P).
+      ℛ ι0 (@SPureSpecM.assert_formulas w0 msg fmls0) (@CPureSpecM.assert_formula P).
     Proof.
-      unfold SDijk.assert_formulas, CDijk.assert_formula.
+      unfold SPureSpecM.assert_formulas, CPureSpecM.assert_formula.
       intros POST__s POST__c HPOST Hwp.
       destruct (solver_spec fmls0) as [[w1 [ζ fmls1]] Hsolver|Hsolver].
       - specialize (Hsolver ι0 Hpc0). destruct Hsolver as [_ Hsolver].
@@ -364,103 +409,145 @@ Module Soundness
       - intuition.
     Qed.
 
-    Lemma approx_assert_formula {w0 : World} (ι0 : Valuation w0) (Hpc0 : instpc (wco w0) ι0)
+    Lemma refine_assert_formula {w0 : World} (ι0 : Valuation w0) (Hpc0 : instpc (wco w0) ι0)
       (msg : AMessage w0) (fml : Formula w0) (P : Prop) (Heq : inst fml ι0 <-> P) :
-      approx ι0 (@SDijk.assert_formula w0 msg fml) (@CDijk.assert_formula P).
-    Proof. unfold SDijk.assert_formula. apply approx_assert_formulas; cbn; intuition. Qed.
+      ℛ ι0 (@SPureSpecM.assert_formula w0 msg fml) (@CPureSpecM.assert_formula P).
+    Proof. unfold SPureSpecM.assert_formula. apply refine_assert_formulas; cbn; intuition. Qed.
 
-    Lemma approx_assert_eq_nenv {N} {Δ : NCtx N Ty} {w0 : World} {ι0 : Valuation w0} (Hpc : instpc (wco w0) ι0)
+    Lemma refine_assert_eq_nenv {N} {Δ : NCtx N Ty} {w0 : World} {ι0 : Valuation w0} (Hpc : instpc (wco w0) ι0)
       (msg : AMessage w0) :
-      approx ι0 (@SDijk.assert_eq_nenv N Δ w0 msg) CDijk.assert_eq_nenv.
+      ℛ ι0 (@SPureSpecM.assert_eq_nenv N Δ w0 msg) CPureSpecM.assert_eq_nenv.
     Proof.
       intros E1 ? -> E2 ? ->.
       induction E1; [ destruct (env.nilView E2) | destruct (env.snocView E2) as [E2] ]; cbn.
-      - now apply approx_pure.
-      - apply approx_bind. apply IHE1.
+      - now apply refine_pure.
+      - apply refine_bind. apply IHE1.
         intros w1 ω01 ι1 -> Hpc1 _ _ _.
-        apply approx_assert_formula; auto. cbn.
+        apply refine_assert_formula; auto. cbn.
         now do 2 rewrite (inst_persist (AT := STerm (type b))).
     Qed.
 
-    Lemma approx_angelic_list {M} `{Subst M, OccursCheck M} {AT A} `{Inst AT A}
+    Lemma refine_assert_eq_env {Δ} {w0 : World} {ι0 : Valuation w0}
+      (Hpc : instpc (wco w0) ι0) (msg : AMessage w0) :
+      ℛ ι0 (@SPureSpecM.assert_eq_env Δ w0 msg) CPureSpecM.assert_eq_env.
+    Proof.
+      intros E1 ? -> E2 ? ->.
+      induction E1; [ destruct (env.nilView E2) | destruct (env.snocView E2) as [E2] ]; cbn.
+      - now apply refine_pure.
+      - apply refine_bind. apply IHE1.
+        intros w1 ω01 ι1 -> Hpc1 _ _ _.
+        apply refine_assert_formula; auto. cbn.
+        now do 2 rewrite (inst_persist (AT := STerm b)).
+    Qed.
+
+    Lemma refine_assert_eq_chunk {w0 : World} {ι0 : Valuation w0} (Hpc : instpc (wco w0) ι0)
+      (msg : AMessage w0) :
+      ℛ ι0 (@SPureSpecM.assert_eq_chunk w0 msg) CPureSpecM.assert_eq_chunk.
+    Proof.
+      intros c ? -> c' ? ->. revert c'.
+      induction c; intros [] w1 ω01 ι1 -> Hpc1; cbn; auto;
+        try (now apply refine_error).
+      - destruct eq_dec.
+        + destruct e; cbn.
+          apply refine_assert_eq_env; auto; cbn;
+            now rewrite <- inst_persist.
+        + now apply refine_error.
+      - destruct eq_dec_het.
+        + dependent elimination e; cbn.
+          apply refine_assert_formula; auto. cbn.
+          now do 2 rewrite <- inst_persist.
+        + now apply refine_error.
+      - apply refine_bind. apply IHc1; auto.
+        intros w2 ω12 ι2 -> Hpc2 _ _ _.
+        apply IHc2; auto.
+        rewrite sub_acc_trans.
+        now rewrite inst_subst, <- inst_persist.
+      - apply refine_bind. apply IHc1; auto.
+        intros w2 ω12 ι2 -> Hpc2 _ _ _.
+        apply IHc2; auto.
+        rewrite sub_acc_trans.
+        now rewrite inst_subst, <- inst_persist.
+    Qed.
+
+    Lemma refine_angelic_list {M} `{Subst M, OccursCheck M} {AT A} `{Inst AT A}
       {w0 : World} (ι0 : Valuation w0) (Hpc0 : instpc (wco w0) ι0) (msg : M w0) :
-      approx ι0 (SDijk.angelic_list (A := AT) msg) (CDijk.angelic_list (A := A)).
+      ℛ ι0 (SPureSpecM.angelic_list (A := AT) msg) (CPureSpecM.angelic_list (A := A)).
     Proof.
       intros xs ? ->.
       induction xs; cbn - [inst];
         intros POST__s POST__c HPOST.
       - intros [].
       - cbn.
-        apply Path.approx_angelic_binary; auto.
+        apply refine_symprop_angelic_binary; auto.
         apply HPOST; wsimpl; auto.
     Qed.
 
-    Lemma approx_demonic_list {AT A} `{Inst AT A}
+    Lemma refine_demonic_list {AT A} `{Inst AT A}
       {w0 : World} (ι0 : Valuation w0) (Hpc0 : instpc (wco w0) ι0) :
-      approx ι0 (@SDijk.demonic_list AT w0) (@CDijk.demonic_list A).
+      ℛ ι0 (@SPureSpecM.demonic_list AT w0) (@CPureSpecM.demonic_list A).
     Proof.
       intros xs ? ->.
       induction xs; cbn - [inst];
         intros POST__s POST__c HPOST.
       - constructor.
       - cbn.
-        apply Path.approx_demonic_binary; auto.
+        apply refine_symprop_demonic_binary; auto.
         apply HPOST; wsimpl; auto.
     Qed.
 
-    Lemma approx_angelic_finite {F} `{finite.Finite F}
+    Lemma refine_angelic_finite {F} `{finite.Finite F}
       {w : World} (ι : Valuation w) (Hpc : instpc (wco w) ι) msg :
-      approx (AT := SDijkstra (Const F)) ι (@SDijk.angelic_finite F _ _ w msg) (@CDijk.angelic_finite F _ _).
+      ℛ (AT := SPureSpecM (Const F)) ι (@SPureSpecM.angelic_finite F _ _ w msg) (@CPureSpecM.angelic_finite F _ _).
     Proof.
-      unfold SDijk.angelic_finite, CDijk.angelic_finite.
-      apply approx_angelic_list; auto.
+      unfold SPureSpecM.angelic_finite, CPureSpecM.angelic_finite.
+      apply refine_angelic_list; auto.
       hnf. unfold inst, inst_const, inst_list.
       now rewrite List.map_id.
     Qed.
 
-    Lemma approx_demonic_finite {F} `{finite.Finite F}
+    Lemma refine_demonic_finite {F} `{finite.Finite F}
       {w : World} (ι : Valuation w) (Hpc : instpc (wco w) ι) :
-      approx (AT := SDijkstra (Const F)) ι (@SDijk.demonic_finite F _ _ w) (@CDijk.demonic_finite F _ _).
+      ℛ (AT := SPureSpecM (Const F)) ι (@SPureSpecM.demonic_finite F _ _ w) (@CPureSpecM.demonic_finite F _ _).
     Proof.
-      unfold SDijk.demonic_finite, CDijk.demonic_finite.
+      unfold SPureSpecM.demonic_finite, CPureSpecM.demonic_finite.
       intros POST__s POST__c HPOST.
-      apply approx_demonic_list; eauto.
+      apply refine_demonic_list; eauto.
       hnf. unfold inst, inst_const, inst_list.
       now rewrite List.map_id.
     Qed.
 
-    (* Lemma approx_angelic_match_bool {w : World} (ι : Valuation w) (Hpc : instpc (wco w) ι) *)
+    (* Lemma refine_angelic_match_bool {w : World} (ι : Valuation w) (Hpc : instpc (wco w) ι) *)
     (*   (msg : Message w) : *)
-    (*   approx ι (@SDijk.angelic_match_bool w msg) (@CDijk.angelic_match_bool). *)
+    (*   ℛ ι (@SPureSpecM.angelic_match_bool w msg) (@CPureSpecM.angelic_match_bool). *)
     (* Proof. *)
     (*   intros t v ->. *)
-    (*   unfold SDijk.angelic_match_bool. *)
+    (*   unfold SPureSpecM.angelic_match_bool. *)
     (*   destruct (term_get_val_spec t). *)
-    (*   - apply approx_pure; auto. *)
-    (*   - unfold SDijk.angelic_match_bool'. *)
+    (*   - apply refine_pure; auto. *)
+    (*   - unfold SPureSpecM.angelic_match_bool'. *)
     (*     intros POST__s POST__c HPOST. *)
-    (*     cbv [SDijk.angelic_binary SDijk.bind CDijk.pure SDijk.assert_formula]. *)
+    (*     cbv [SPureSpecM.angelic_binary SPureSpecM.bind CPureSpecM.pure SPureSpecM.assert_formula]. *)
     (*     hnf. *)
     (*     intros δs δc Hδ hs hc Hh. *)
-    (*     hnf. rewrite CMut.wp_angelic_match_bool. *)
+    (*     hnf. rewrite CHeapSpecM.wp_angelic_match_bool. *)
     (*     destruct a. *)
     (*     + apply Hkt; wsimpl; eauto. *)
     (*     + apply Hkf; wsimpl; eauto. *)
-    (*   - now apply approx_angelic_match_bool'. *)
+    (*   - now apply refine_angelic_match_bool'. *)
     (* Qed. *)
 
-  End Dijk.
+  End PureSpecM.
 
   Section Basics.
 
-    Lemma approx_dijkstra {Γ AT A} `{Approx AT A}
+    Lemma refine_lift_purem {Γ AT A} `{Refine AT A}
       {w0 : World} (ι0 : Valuation w0) (Hpc0 : instpc (wco w0) ι0) :
-      approx ι0 (@SMut.dijkstra Γ AT w0) (@CMut.dijkstra Γ A).
+      ℛ ι0 (@SHeapSpecM.lift_purem Γ AT w0) (@CHeapSpecM.lift_purem Γ A).
     Proof.
       intros ms mc Hm.
       intros POST__s POST__c HPOST.
       intros δs δc Hδ hs hc Hh.
-      unfold SMut.dijkstra, CMut.dijkstra.
+      unfold SHeapSpecM.lift_purem, CHeapSpecM.lift_purem.
       apply Hm.
       intros w1 ω01 ι1 -> Hpc1.
       intros a1 a Ha.
@@ -468,65 +555,65 @@ Module Soundness
       hnf. rewrite inst_persist. apply Hδ.
       hnf. rewrite inst_persist. apply Hh.
     Qed.
-    Hint Resolve approx_dijkstra : core.
+    Hint Resolve refine_lift_purem : core.
 
-    Lemma approx_block {AT A} `{Approx AT A} {Γ1 Γ2} {w : World} (ι : Valuation w) :
-      approx ι (@SMut.block Γ1 Γ2 AT w) CMut.block.
-    Proof. unfold approx, ApproxMut, ApproxImpl. auto. Qed.
+    Lemma refine_block {AT A} `{Refine AT A} {Γ1 Γ2} {w : World} (ι : Valuation w) :
+      ℛ ι (@SHeapSpecM.block Γ1 Γ2 AT w) CHeapSpecM.block.
+    Proof. unfold ℛ, RefineHeapSpecM, RefineImpl. auto. Qed.
 
-    Lemma approx_error {AT A D} `{Approx AT A} {Γ1 Γ2} {w : World} {ι: Valuation w} (func msg : string) (d : D) (cm : CMut Γ1 Γ2 A) :
-      approx ι (@SMut.error Γ1 Γ2 AT D func msg d w) cm.
+    Lemma refine_error {AT A D} `{Refine AT A} {Γ1 Γ2} {w : World} {ι: Valuation w} (func msg : string) (d : D) (cm : CHeapSpecM Γ1 Γ2 A) :
+      ℛ ι (@SHeapSpecM.error Γ1 Γ2 AT D func msg d w) cm.
     Proof.
       intros POST__s POST__c HPOST.
       intros δs δc Hδ hs hc Hh [].
     Qed.
-    Hint Resolve approx_error : core.
+    Hint Resolve refine_error : core.
 
-    Lemma approx_pure {AT A} `{Approx AT A} {Γ} {w : World} (ι : Valuation w) (Hpc : instpc (wco w) ι) :
-      approx ι (@SMut.pure Γ AT w) CMut.pure.
+    Lemma refine_pure {AT A} `{Refine AT A} {Γ} {w : World} (ι : Valuation w) (Hpc : instpc (wco w) ι) :
+      ℛ ι (@SHeapSpecM.pure Γ AT w) CHeapSpecM.pure.
     Proof.
       intros t v tv.
       intros POST__s POST__c HPOST.
-      unfold SMut.pure, CMut.pure.
+      unfold SHeapSpecM.pure, CHeapSpecM.pure.
       apply HPOST; auto. cbn.
       now rewrite inst_sub_id.
     Qed.
 
-    Lemma approx_bind {AT A BT B} `{Approx AT A, Approx BT B}
+    Lemma refine_bind {AT A BT B} `{Refine AT A, Refine BT B}
       {Γ1 Γ2 Γ3} {w0 : World} (ι0 : Valuation w0) (* (Hpc0 : instpc (wco w0) ι0) *) :
-      approx ι0 (@SMut.bind Γ1 Γ2 Γ3 AT BT w0) (@CMut.bind Γ1 Γ2 Γ3 A B).
+      ℛ ι0 (@SHeapSpecM.bind Γ1 Γ2 Γ3 AT BT w0) (@CHeapSpecM.bind Γ1 Γ2 Γ3 A B).
     Proof.
-      (* cbv [approx ApproxBox ApproxImpl ApproxMut ApproxPath ApproxInst]. *)
+      (* cbv [ℛ RefineBox RefineImpl RefineHeapSpecM RefineProp RefineInst]. *)
       intros ms mc Hm fs fc Hf.
       intros POST__s POST__c HPOST.
       intros δs δc -> hs hc ->.
-      unfold SMut.bind, CMut.bind.
+      unfold SHeapSpecM.bind, CHeapSpecM.bind.
       apply Hm; eauto.
       intros w1 ω01 ι1 -> Hpc1.
       intros a1 a Ha.
       apply Hf; auto.
-      eapply approx_four; eauto.
+      eapply refine_four; eauto.
     Qed.
 
-    Lemma approx_bind_right {AT A BT B} `{Approx AT A, Approx BT B}
-      {Γ1 Γ2 Γ3} {w0 : World} (ι0 : Valuation w0) (* (Hpc0 : instpc (wco w0) ι0) *) :
-      approx ι0 (@SMut.bind_right Γ1 Γ2 Γ3 AT BT w0) (@CMut.bind_right Γ1 Γ2 Γ3 A B).
-    Proof.
-      intros ms1 mc1 Hm1 ms2 mc2 Hm2.
-      intros POST__s POST__c HPOST.
-      intros δs δc -> hs hc ->.
-      unfold SMut.bind_right, CMut.bind_right, CMut.bind.
-      apply Hm1; eauto.
-      intros w1 ω01 ι1 -> Hpc1.
-      intros a1 a Ha.
-      apply Hm2; auto.
-      eapply approx_four; eauto.
-    Qed.
+    (* Lemma refine_bind_right {AT A BT B} `{Refine AT A, Refine BT B} *)
+    (*   {Γ1 Γ2 Γ3} {w0 : World} (ι0 : Valuation w0) (* (Hpc0 : instpc (wco w0) ι0) *) : *)
+    (*   ℛ ι0 (@SHeapSpecM.bind_right Γ1 Γ2 Γ3 AT BT w0) (@CHeapSpecM.bind_right Γ1 Γ2 Γ3 A B). *)
+    (* Proof. *)
+    (*   intros ms1 mc1 Hm1 ms2 mc2 Hm2. *)
+    (*   intros POST__s POST__c HPOST. *)
+    (*   intros δs δc -> hs hc ->. *)
+    (*   unfold SHeapSpecM.bind_right, CHeapSpecM.bind_right, CHeapSpecM.bind. *)
+    (*   apply Hm1; eauto. *)
+    (*   intros w1 ω01 ι1 -> Hpc1. *)
+    (*   intros a1 a Ha. *)
+    (*   apply Hm2; auto. *)
+    (*   eapply refine_four; eauto. *)
+    (* Qed. *)
 
-    Lemma approx_angelic (x : option 𝑺) (σ : Ty)
+    Lemma refine_angelic (x : option 𝑺) (σ : Ty)
       {Γ : PCtx} {w0 : World} (ι0 : Valuation w0)
       (Hpc0 : instpc (wco w0) ι0) :
-      approx ι0 (@SMut.angelic Γ x σ w0) (@CMut.angelic Γ σ).
+      ℛ ι0 (@SHeapSpecM.angelic Γ x σ w0) (@CHeapSpecM.angelic Γ σ).
     Proof.
       intros POST__s POST__c HPOST.
       intros δs δc -> hs hc ->.
@@ -537,12 +624,12 @@ Module Soundness
       hnf. cbn. now rewrite inst_subst, ?inst_sub_wk1.
       hnf. cbn. now rewrite inst_subst, ?inst_sub_wk1.
     Qed.
-    Hint Resolve approx_angelic : core.
+    Hint Resolve refine_angelic : core.
 
-    Lemma approx_demonic (x : option 𝑺) (σ : Ty)
+    Lemma refine_demonic (x : option 𝑺) (σ : Ty)
       {Γ : PCtx} {w0 : World} (ι0 : Valuation w0)
       (Hpc0 : instpc (wco w0) ι0) :
-      approx ι0 (@SMut.demonic Γ x σ w0) (@CMut.demonic Γ σ).
+      ℛ ι0 (@SHeapSpecM.demonic Γ x σ w0) (@CHeapSpecM.demonic Γ σ).
     Proof.
       intros POST__s POST__c HPOST.
       intros δs δc -> hs hc ->.
@@ -553,187 +640,199 @@ Module Soundness
       hnf. cbn. now rewrite inst_subst, ?inst_sub_wk1.
       hnf. cbn. now rewrite inst_subst, ?inst_sub_wk1.
     Qed.
-    Hint Resolve approx_demonic : core.
+    Hint Resolve refine_demonic : core.
 
-    Lemma approx_angelic_ctx {N : Set} (n : N -> 𝑺) {Γ : PCtx} (Δ : NCtx N Ty) :
+    Lemma refine_angelic_ctx {N : Set} (n : N -> 𝑺) {Γ : PCtx} (Δ : NCtx N Ty) :
       forall {w0 : World} (ι0 : Valuation w0) (Hpc0 : instpc (wco w0) ι0),
-        approx ι0 (@SMut.angelic_ctx N n Γ w0 Δ) (@CMut.angelic_ctx N Γ Δ).
+        ℛ ι0 (@SHeapSpecM.angelic_ctx N n Γ w0 Δ) (@CHeapSpecM.angelic_ctx N Γ Δ).
     Proof.
-      intros w0 ι0 Hpc0. unfold SMut.angelic_ctx, CMut.angelic_ctx.
-      apply approx_dijkstra; auto.
-      now apply Dijk.approx_angelic_ctx.
+      intros w0 ι0 Hpc0. unfold SHeapSpecM.angelic_ctx, CHeapSpecM.angelic_ctx.
+      apply refine_lift_purem; auto.
+      now apply PureSpecM.refine_angelic_ctx.
     Qed.
 
-    Lemma approx_demonic_ctx {N : Set} (n : N -> 𝑺) {Γ : PCtx} (Δ : NCtx N Ty) :
+    Lemma refine_demonic_ctx {N : Set} (n : N -> 𝑺) {Γ : PCtx} (Δ : NCtx N Ty) :
       forall {w0 : World} (ι0 : Valuation w0) (Hpc0 : instpc (wco w0) ι0),
-        approx ι0 (@SMut.demonic_ctx N n Γ w0 Δ) (@CMut.demonic_ctx N Γ Δ).
+        ℛ ι0 (@SHeapSpecM.demonic_ctx N n Γ w0 Δ) (@CHeapSpecM.demonic_ctx N Γ Δ).
     Proof.
-      intros w0 ι0 Hpc0. unfold SMut.demonic_ctx, CMut.demonic_ctx.
-      apply approx_dijkstra; auto.
-      now apply Dijk.approx_demonic_ctx.
+      intros w0 ι0 Hpc0. unfold SHeapSpecM.demonic_ctx, CHeapSpecM.demonic_ctx.
+      apply refine_lift_purem; auto.
+      now apply PureSpecM.refine_demonic_ctx.
     Qed.
 
-    Lemma approx_debug {AT A D} `{Approx AT A, Subst D, SubstLaws D, OccursCheck D} {Γ1 Γ2} {w0 : World} (ι0 : Valuation w0)
+    Lemma refine_debug {AT A D} `{Refine AT A, Subst D, SubstLaws D, OccursCheck D} {Γ1 Γ2} {w0 : World} (ι0 : Valuation w0)
           (Hpc : instpc (wco w0) ι0) f ms mc :
-      approx ι0 ms mc ->
-      approx ι0 (@SMut.debug AT D _ _ _ _ Γ1 Γ2 w0 f ms) mc.
+      ℛ ι0 ms mc ->
+      ℛ ι0 (@SHeapSpecM.debug AT D _ _ _ _ Γ1 Γ2 w0 f ms) mc.
     Proof.
       intros Hap.
       intros POST__s POST__c HPOST.
       intros δs0 δc0 -> hs0 hc0 ->.
-      unfold SMut.debug. hnf.
+      unfold SHeapSpecM.debug. hnf.
       cbn. intros [HP]. revert HP.
       apply Hap; auto.
     Qed.
 
-    Lemma approx_angelic_binary {AT A} `{Approx AT A} {Γ1 Γ2} {w : World} (ι : Valuation w) :
-      approx ι (@SMut.angelic_binary Γ1 Γ2 AT w) (@CMut.angelic_binary Γ1 Γ2 A).
+    Lemma refine_angelic_binary {AT A} `{Refine AT A} {Γ1 Γ2} {w : World} (ι : Valuation w) :
+      ℛ ι (@SHeapSpecM.angelic_binary Γ1 Γ2 AT w) (@CHeapSpecM.angelic_binary Γ1 Γ2 A).
     Proof.
       intros ms1 mc1 Hm1 ms2 mc2 Hm2.
       intros POST__s POST__c HPOST.
       intros δs0 δc0 -> hs0 hc0 ->.
-      unfold SMut.angelic_binary, CMut.angelic_binary.
+      unfold SHeapSpecM.angelic_binary, CHeapSpecM.angelic_binary.
       intros [HYP|HYP]; [left|right]; revert HYP.
       - apply Hm1; auto.
       - apply Hm2; auto.
     Qed.
 
-    Lemma approx_demonic_binary {AT A} `{Approx AT A} {Γ1 Γ2} {w : World} (ι : Valuation w) :
-      approx ι (@SMut.demonic_binary Γ1 Γ2 AT w) (@CMut.demonic_binary Γ1 Γ2 A).
+    Lemma refine_demonic_binary {AT A} `{Refine AT A} {Γ1 Γ2} {w : World} (ι : Valuation w) :
+      ℛ ι (@SHeapSpecM.demonic_binary Γ1 Γ2 AT w) (@CHeapSpecM.demonic_binary Γ1 Γ2 A).
     Proof.
       intros ms1 mc1 Hm1 ms2 mc2 Hm2.
       intros POST__s POST__c HPOST.
       intros δs0 δc0 -> hs0 hc0 ->.
-      unfold SMut.demonic_binary, CMut.demonic_binary.
+      unfold SHeapSpecM.demonic_binary, CHeapSpecM.demonic_binary.
       intros [H1 H2]. split.
       - revert H1. apply Hm1; auto.
       - revert H2. apply Hm2; auto.
     Qed.
 
-    Lemma approx_angelic_list {M} {subM : Subst M} {occM : OccursCheck M} {AT A} `{Inst AT A} {Γ}
+    Lemma refine_angelic_list {M} {subM : Subst M} {occM : OccursCheck M} {AT A} `{Inst AT A} {Γ}
       {w : World} (ι : Valuation w) (Hpc : instpc (wco w) ι)
       (msg : SStore Γ w -> SHeap w -> M w) :
-      approx ι (SMut.angelic_list (A := AT) msg) (@CMut.angelic_list A Γ).
+      ℛ ι (SHeapSpecM.angelic_list (A := AT) msg) (@CHeapSpecM.angelic_list A Γ).
     Proof.
       intros ls lc Hl.
-      unfold SMut.angelic_list, CMut.angelic_list.
+      unfold SHeapSpecM.angelic_list, CHeapSpecM.angelic_list.
       intros POST__s POST__c HPOST.
       intros δs0 δc0 Hδ0 hs0 hc0 Hh0.
-      apply approx_dijkstra; eauto.
-      apply Dijk.approx_angelic_list; auto.
+      apply refine_lift_purem; eauto.
+      apply PureSpecM.refine_angelic_list; auto.
     Qed.
 
-    Lemma approx_angelic_finite {F} `{finite.Finite F} {Γ}
+    Lemma refine_angelic_finite {F} `{finite.Finite F} {Γ}
       {w : World} (ι : Valuation w) (Hpc : instpc (wco w) ι) msg :
-      approx (AT := SMut Γ Γ (Const F)) ι (@SMut.angelic_finite Γ F _ _ w msg) (@CMut.angelic_finite Γ F _ _).
+      ℛ (AT := SHeapSpecM Γ Γ (Const F)) ι (@SHeapSpecM.angelic_finite Γ F _ _ w msg) (@CHeapSpecM.angelic_finite Γ F _ _).
     Proof.
-      unfold SMut.angelic_finite, CMut.angelic_finite.
+      unfold SHeapSpecM.angelic_finite, CHeapSpecM.angelic_finite.
       intros POST__s POST__c HPOST.
       intros δs0 δc0 Hδ0 hs0 hc0 Hh0.
-      eapply approx_dijkstra; eauto.
-      apply Dijk.approx_angelic_finite; auto.
+      apply refine_lift_purem; eauto.
+      apply PureSpecM.refine_angelic_finite; auto.
     Qed.
 
-    Lemma approx_demonic_finite {F} `{finite.Finite F} {Γ}
+    Lemma refine_demonic_finite {F} `{finite.Finite F} {Γ}
       {w : World} (ι : Valuation w) (Hpc : instpc (wco w) ι) :
-      approx (AT := SMut Γ Γ (Const F)) ι (@SMut.demonic_finite Γ F _ _ w) (@CMut.demonic_finite Γ F _ _).
+      ℛ (AT := SHeapSpecM Γ Γ (Const F)) ι (@SHeapSpecM.demonic_finite Γ F _ _ w) (@CHeapSpecM.demonic_finite Γ F _ _).
     Proof.
-      unfold SMut.demonic_finite, CMut.demonic_finite.
+      unfold SHeapSpecM.demonic_finite, CHeapSpecM.demonic_finite.
       intros POST__s POST__c HPOST.
       intros δs0 δc0 Hδ0 hs0 hc0 Hh0.
-      eapply approx_dijkstra; eauto.
-      apply Dijk.approx_demonic_finite; auto.
+      apply refine_lift_purem; eauto.
+      apply PureSpecM.refine_demonic_finite; auto.
     Qed.
 
   End Basics.
 
   Section AssumeAssert.
 
-    Lemma approx_assume_formula {Γ} {w0 : World} {ι0 : Valuation w0} (Hpc0 : instpc (wco w0) ι0)
+    Lemma refine_assume_formula {Γ} {w0 : World} {ι0 : Valuation w0} (Hpc0 : instpc (wco w0) ι0)
       (fml__s : Formula w0) (fml__c : Prop) (Hfml : fml__c <-> inst fml__s ι0) :
-      approx ι0 (@SMut.assume_formula Γ w0 fml__s) (CMut.assume_formula fml__c).
+      ℛ ι0 (@SHeapSpecM.assume_formula Γ w0 fml__s) (CHeapSpecM.assume_formula fml__c).
     Proof.
-      unfold SMut.assume_formula, CMut.assume_formula.
-      apply approx_dijkstra; auto.
-      now apply Dijk.approx_assume_formula.
+      unfold SHeapSpecM.assume_formula, CHeapSpecM.assume_formula.
+      apply refine_lift_purem; auto.
+      now apply PureSpecM.refine_assume_formula.
     Qed.
 
-    Lemma approx_box_assume_formula {Γ} {w0 : World} {ι0 : Valuation w0} (Hpc0 : instpc (wco w0) ι0)
+    Lemma refine_box_assume_formula {Γ} {w0 : World} {ι0 : Valuation w0} (Hpc0 : instpc (wco w0) ι0)
       (fml__s : Formula w0) (fml__c : Prop) (Hfml : fml__c <-> inst fml__s ι0) :
-      approx ι0 (@SMut.box_assume_formula Γ w0 fml__s) (CMut.assume_formula fml__c).
+      ℛ ι0 (@SHeapSpecM.box_assume_formula Γ w0 fml__s) (CHeapSpecM.assume_formula fml__c).
     Proof.
-      unfold SMut.box_assume_formula, fmap_box.
+      unfold SHeapSpecM.box_assume_formula, fmap_box.
       intros w1 ω01 ι1 -> Hpc1.
-      apply approx_assume_formula; auto.
+      apply refine_assume_formula; auto.
       now rewrite inst_persist.
     Qed.
 
-    Lemma approx_assert_formula {Γ} {w0 : World} (ι0 : Valuation w0) (Hpc : instpc (wco w0) ι0)
+    Lemma refine_assert_formula {Γ} {w0 : World} (ι0 : Valuation w0) (Hpc : instpc (wco w0) ι0)
       (fml__s : Formula w0) (fml__c : Prop) (Hfml : fml__c <-> inst fml__s ι0) :
-      approx ι0 (@SMut.assert_formula Γ w0 fml__s) (@CMut.assert_formula Γ fml__c).
+      ℛ ι0 (@SHeapSpecM.assert_formula Γ w0 fml__s) (@CHeapSpecM.assert_formula Γ fml__c).
     Proof.
-      unfold SMut.assert_formula, CMut.assert_formula.
+      unfold SHeapSpecM.assert_formula, CHeapSpecM.assert_formula.
       intros POST__s POST__c HPOST.
       intros δs δc Hδ hs hc Hh.
-      apply approx_dijkstra; auto.
-      now apply Dijk.approx_assert_formula.
+      apply refine_lift_purem; auto.
+      now apply PureSpecM.refine_assert_formula.
     Qed.
 
-    Lemma approx_box_assert_formula {Γ} {w0 : World} {ι0 : Valuation w0} (Hpc0 : instpc (wco w0) ι0)
+    Lemma refine_box_assert_formula {Γ} {w0 : World} {ι0 : Valuation w0} (Hpc0 : instpc (wco w0) ι0)
       (fml__s : Formula w0) (fml__c : Prop) (Hfml : fml__c <-> inst fml__s ι0) :
-      approx ι0 (@SMut.box_assert_formula Γ w0 fml__s) (CMut.assert_formula fml__c).
+      ℛ ι0 (@SHeapSpecM.box_assert_formula Γ w0 fml__s) (CHeapSpecM.assert_formula fml__c).
     Proof.
-      unfold SMut.box_assert_formula, fmap_box.
+      unfold SHeapSpecM.box_assert_formula, fmap_box.
       intros w1 ω01 ι1 -> Hpc1.
-      apply approx_assert_formula; auto.
+      apply refine_assert_formula; auto.
       now rewrite inst_persist.
     Qed.
 
-    Lemma approx_assert_formulas {Γ} {w0 : World} (ι0 : Valuation w0) (Hpc : instpc (wco w0) ι0)
+    Lemma refine_assert_formulas {Γ} {w0 : World} (ι0 : Valuation w0) (Hpc : instpc (wco w0) ι0)
       (fmls__s : List Formula w0) (fmls__c : Prop) (Hfmls : fmls__c <-> instpc fmls__s ι0) :
-      approx ι0 (@SMut.assert_formulas Γ w0 fmls__s) (@CMut.assert_formula Γ fmls__c).
+      ℛ ι0 (@SHeapSpecM.assert_formulas Γ w0 fmls__s) (@CHeapSpecM.assert_formula Γ fmls__c).
     Proof.
       intros POST__s POST__c HPOST.
       intros δs δc -> hs hc ->.
-      unfold SMut.assert_formulas, CMut.assert_formula.
-      apply approx_dijkstra; auto.
-      now apply Dijk.approx_assert_formulas.
+      unfold SHeapSpecM.assert_formulas, CHeapSpecM.assert_formula.
+      apply refine_lift_purem; auto.
+      now apply PureSpecM.refine_assert_formulas.
     Qed.
 
-    Lemma approx_assert_eq_nenv {N Γ} (Δ : NCtx N Ty) {w0 : World} (ι0 : Valuation w0) (Hpc : instpc (wco w0) ι0) :
-      approx ι0 (@SMut.assert_eq_nenv N Γ Δ w0) (@CMut.assert_eq_nenv N Γ Δ).
+    Lemma refine_assert_eq_nenv {N Γ} (Δ : NCtx N Ty) {w0 : World} (ι0 : Valuation w0) (Hpc : instpc (wco w0) ι0) :
+      ℛ ι0 (@SHeapSpecM.assert_eq_nenv N Γ Δ w0) (@CHeapSpecM.assert_eq_nenv N Γ Δ).
     Proof.
       intros E1 ? ? E2 ? ? POST__s POST__c HPOST δs δc -> hs hc ->.
-      unfold SMut.assert_eq_nenv, CMut.assert_eq_nenv.
-      apply approx_dijkstra; auto.
-      apply Dijk.approx_assert_eq_nenv; auto.
+      unfold SHeapSpecM.assert_eq_nenv, CHeapSpecM.assert_eq_nenv.
+      apply refine_lift_purem; auto.
+      apply PureSpecM.refine_assert_eq_nenv; auto.
+    Qed.
+
+    Lemma refine_assert_eq_chunk {Γ} {w0 : World} {ι0 : Valuation w0} (Hpc : instpc (wco w0) ι0) :
+      ℛ ι0 (@SHeapSpecM.assert_eq_chunk Γ w0) CHeapSpecM.assert_eq_chunk.
+    Proof.
+      intros c1 ? ? E2 ? ? POST__s POST__c HPOST δs δc Hδ hs hc Hh.
+      unfold SHeapSpecM.assert_eq_chunk, CHeapSpecM.assert_eq_chunk.
+      apply refine_lift_purem; auto. unfold T.
+      eapply PureSpecM.refine_assert_eq_chunk; cbn; eauto.
+      now rewrite inst_sub_id.
     Qed.
 
   End AssumeAssert.
 
   Section PatternMatching.
 
-    Lemma approx_angelic_match_bool' {AT A} `{Approx AT A} {Γ1 Γ2}
+    Lemma refine_angelic_match_bool' {AT A} `{Refine AT A} {Γ1 Γ2}
       {w : World} (ι : Valuation w) (Hpc: instpc (wco w) ι) :
-      approx ι (@SMut.angelic_match_bool' AT Γ1 Γ2 w) (CMut.angelic_match_bool (A := A)).
+      ℛ ι (@SHeapSpecM.angelic_match_bool' AT Γ1 Γ2 w) (CHeapSpecM.angelic_match_bool (A := A)).
     Proof.
-      unfold SMut.angelic_match_bool', CMut.angelic_match_bool.
+      unfold SHeapSpecM.angelic_match_bool', CHeapSpecM.angelic_match_bool.
       intros t v ->.
       intros kt__s kt__c Hkt.
       intros kf__s kf__c Hkf.
-      apply approx_angelic_binary; eauto.
-      apply approx_bind_right; eauto.
-      apply approx_assert_formula; eauto.
-      apply approx_bind_right; eauto.
-      apply approx_assert_formula; eauto.
-      cbn. unfold is_true. now rewrite negb_true_iff.
+      apply refine_angelic_binary; eauto.
+      - apply refine_bind; eauto.
+        apply refine_assert_formula; eauto.
+        intros ? ? ? -> ? _ _ _. auto.
+      - apply refine_bind; eauto.
+        apply refine_assert_formula; eauto.
+        cbn. unfold is_true. now rewrite negb_true_iff.
+        intros ? ? ? -> ? _ _ _. auto.
     Qed.
 
-    Lemma approx_angelic_match_bool {AT A} `{Approx AT A} {Γ1 Γ2}
+    Lemma refine_angelic_match_bool {AT A} `{Refine AT A} {Γ1 Γ2}
       {w : World} (ι : Valuation w) (Hpc : instpc (wco w) ι) :
-      approx ι (@SMut.angelic_match_bool AT Γ1 Γ2 w) (CMut.angelic_match_bool (A := A)).
+      ℛ ι (@SHeapSpecM.angelic_match_bool AT Γ1 Γ2 w) (CHeapSpecM.angelic_match_bool (A := A)).
     Proof.
-      unfold SMut.angelic_match_bool.
+      unfold SHeapSpecM.angelic_match_bool.
       intros t v ->.
       destruct (term_get_val_spec t).
       - rewrite H0.
@@ -741,47 +840,49 @@ Module Soundness
         intros kf__s kf__c Hkf.
         intros POST__s POST__c HPOST.
         intros δs δc Hδ hs hc Hh.
-        hnf. rewrite CMut.wp_angelic_match_bool.
+        hnf. rewrite CHeapSpecM.wp_angelic_match_bool.
         destruct a.
         + apply Hkt; wsimpl; eauto.
         + apply Hkf; wsimpl; eauto.
-      - now apply approx_angelic_match_bool'.
+      - now apply refine_angelic_match_bool'.
     Qed.
 
-    Lemma approx_box_angelic_match_bool {AT A} `{Approx AT A} {Γ1 Γ2}
+    Lemma refine_box_angelic_match_bool {AT A} `{Refine AT A} {Γ1 Γ2}
       {w : World} (ι : Valuation w) :
-      approx ι (@SMut.box_angelic_match_bool AT Γ1 Γ2 w) (CMut.angelic_match_bool (A := A)).
+      ℛ ι (@SHeapSpecM.box_angelic_match_bool AT Γ1 Γ2 w) (CHeapSpecM.angelic_match_bool (A := A)).
     Proof.
-      unfold SMut.box_angelic_match_bool, fmap_box, K.
+      unfold SHeapSpecM.box_angelic_match_bool, fmap_box, K.
       intros t v ->.
       intros kt__s kt__c Hkt.
       intros kf__s kf__c Hkf.
       intros w1 ω01 ι1 -> Hpc1.
-      apply approx_angelic_match_bool; wsimpl; eauto.
+      apply refine_angelic_match_bool; wsimpl; eauto.
       rewrite <- inst_persist; auto.
     Qed.
 
-    Lemma approx_demonic_match_bool' {AT A} `{Approx AT A} {Γ1 Γ2}
+    Lemma refine_demonic_match_bool' {AT A} `{Refine AT A} {Γ1 Γ2}
       {w : World} (ι : Valuation w) (Hpc : instpc (wco w) ι) :
-      approx ι (@SMut.demonic_match_bool' AT Γ1 Γ2 w) (CMut.demonic_match_bool (A := A)).
+      ℛ ι (@SHeapSpecM.demonic_match_bool' AT Γ1 Γ2 w) (CHeapSpecM.demonic_match_bool (A := A)).
     Proof.
-      unfold SMut.demonic_match_bool, CMut.demonic_match_bool.
+      unfold SHeapSpecM.demonic_match_bool, CHeapSpecM.demonic_match_bool.
       intros t v ->.
       intros kt__s kt__c Hkt.
       intros kf__s kf__c Hkf.
-      apply approx_demonic_binary; eauto.
-      apply approx_bind_right; eauto.
-      apply approx_assume_formula; eauto.
-      apply approx_bind_right; eauto.
-      apply approx_assume_formula; eauto.
-      cbn. unfold is_true. now rewrite negb_true_iff.
+      apply refine_demonic_binary; eauto.
+      - apply refine_bind; eauto.
+        apply refine_assume_formula; eauto.
+        intros ? ? ? -> ? _ _ _. auto.
+      - apply refine_bind; eauto.
+        apply refine_assume_formula; eauto.
+        cbn. unfold is_true. now rewrite negb_true_iff.
+        intros ? ? ? -> ? _ _ _. auto.
     Qed.
 
-    Lemma approx_demonic_match_bool {AT A} `{Approx AT A} {Γ1 Γ2} {w : World}
+    Lemma refine_demonic_match_bool {AT A} `{Refine AT A} {Γ1 Γ2} {w : World}
       (ι : Valuation w) (Hpc : instpc (wco w) ι) :
-      approx ι (@SMut.demonic_match_bool AT Γ1 Γ2 w) (CMut.demonic_match_bool (A := A)).
+      ℛ ι (@SHeapSpecM.demonic_match_bool AT Γ1 Γ2 w) (CHeapSpecM.demonic_match_bool (A := A)).
     Proof.
-      unfold SMut.demonic_match_bool.
+      unfold SHeapSpecM.demonic_match_bool.
       intros t v ->.
       destruct (term_get_val_spec t).
       - rewrite H0.
@@ -789,338 +890,344 @@ Module Soundness
         intros kf__s kf__c Hkf.
         intros POST__s POST__c HPOST.
         intros δs δc Hδ hs hc Hh.
-        hnf. rewrite CMut.wp_demonic_match_bool.
+        hnf. rewrite CHeapSpecM.wp_demonic_match_bool.
         destruct a.
         + apply Hkt; wsimpl; eauto.
         + apply Hkf; wsimpl; eauto.
-      - now apply approx_demonic_match_bool'.
+      - now apply refine_demonic_match_bool'.
     Qed.
 
-    Lemma approx_box_demonic_match_bool {AT A} `{Approx AT A} {Γ1 Γ2}
+    Lemma refine_box_demonic_match_bool {AT A} `{Refine AT A} {Γ1 Γ2}
       {w : World} (ι : Valuation w) (Hpc : instpc (wco w) ι) :
-      approx ι (@SMut.box_demonic_match_bool AT Γ1 Γ2 w) (CMut.demonic_match_bool (A := A)).
+      ℛ ι (@SHeapSpecM.box_demonic_match_bool AT Γ1 Γ2 w) (CHeapSpecM.demonic_match_bool (A := A)).
     Proof.
-      unfold SMut.box_demonic_match_bool, fmap_box, K.
+      unfold SHeapSpecM.box_demonic_match_bool, fmap_box, K.
       intros t v ->.
       intros kt__s kt__c Hkt.
       intros kf__s kf__c Hkf.
       intros w1 ω01 ι1 -> Hpc1.
-      apply approx_demonic_match_bool; wsimpl; eauto.
+      apply refine_demonic_match_bool; wsimpl; eauto.
       rewrite <- inst_persist. auto.
     Qed.
 
-    Lemma approx_angelic_match_enum {AT A} `{Approx AT A} {E : enumi} {Γ1 Γ2 : PCtx}
+    Lemma refine_angelic_match_enum {AT A} `{Refine AT A} {E : enumi} {Γ1 Γ2 : PCtx}
       {w : World} (ι : Valuation w) (Hpc : instpc (wco w) ι) :
-      approx ι (@SMut.angelic_match_enum AT E Γ1 Γ2 w) (@CMut.angelic_match_enum A E Γ1 Γ2).
+      ℛ ι (@SHeapSpecM.angelic_match_enum AT E Γ1 Γ2 w) (@CHeapSpecM.angelic_match_enum A E Γ1 Γ2).
     Proof.
       intros t v ->.
       intros ks kc Hk.
-      unfold SMut.angelic_match_enum, CMut.angelic_match_enum.
-      apply approx_bind.
-      apply approx_angelic_finite; auto.
+      unfold SHeapSpecM.angelic_match_enum, CHeapSpecM.angelic_match_enum.
+      apply refine_bind.
+      apply refine_angelic_finite; auto.
       intros w1 ω01 ι1 -> Hpc1.
       intros EK1 EK2 ->.
-      apply approx_bind_right.
-      apply approx_assert_formula; cbn; wsimpl; auto.
+      apply refine_bind.
+      apply refine_assert_formula; cbn; wsimpl; auto.
       now rewrite <- inst_persist.
-      intros w2 ω12 ι2 -> Hpc2.
-      eapply Hk; wsimpl; auto.
+      intros w2 ω12 ι2 -> Hpc2 _ _ _.
+      apply Hk; wsimpl; auto.
     Qed.
 
-    Lemma approx_demonic_match_enum {AT A} `{Approx AT A} {E : enumi} {Γ1 Γ2 : PCtx}
+    Lemma refine_demonic_match_enum {AT A} `{Refine AT A} {E : enumi} {Γ1 Γ2 : PCtx}
       {w : World} (ι : Valuation w) (Hpc : instpc (wco w) ι) :
-      approx ι (@SMut.demonic_match_enum AT E Γ1 Γ2 w) (@CMut.demonic_match_enum A E Γ1 Γ2).
+      ℛ ι (@SHeapSpecM.demonic_match_enum AT E Γ1 Γ2 w) (@CHeapSpecM.demonic_match_enum A E Γ1 Γ2).
     Proof.
       intros t v ->.
       intros ks kc Hk.
-      unfold SMut.demonic_match_enum, CMut.demonic_match_enum.
-      apply approx_bind.
-      apply approx_demonic_finite; auto.
+      unfold SHeapSpecM.demonic_match_enum, CHeapSpecM.demonic_match_enum.
+      apply refine_bind.
+      apply refine_demonic_finite; auto.
       intros w1 ω01 ι1 -> Hpc1.
       intros EK1 EK2 ->.
-      apply approx_bind_right.
-      apply approx_assume_formula; cbn; wsimpl; auto.
+      apply refine_bind.
+      apply refine_assume_formula; cbn; wsimpl; auto.
       now rewrite <- inst_persist.
-      intros w2 ω12 ι2 -> Hpc2.
-      eapply Hk; wsimpl; auto.
+      intros w2 ω12 ι2 -> Hpc2 _ _ _.
+      apply Hk; wsimpl; auto.
     Qed.
 
-    Lemma approx_angelic_match_sum {AT A} `{Approx AT A} {Γ1 Γ2} x y σ τ
+    Lemma refine_angelic_match_sum {AT A} `{Refine AT A} {Γ1 Γ2} x y σ τ
       {w : World} (ι : Valuation w) (Hpc : instpc (wco w) ι) :
-      approx ι (@SMut.angelic_match_sum AT Γ1 Γ2 x y σ τ w) (@CMut.angelic_match_sum A Γ1 Γ2 σ τ).
+      ℛ ι (@SHeapSpecM.angelic_match_sum AT Γ1 Γ2 x y σ τ w) (@CHeapSpecM.angelic_match_sum A Γ1 Γ2 σ τ).
     Proof.
       intros t v ->.
       intros kl kl__c Hk__l.
       intros kr kr__c Hk__r.
-      unfold SMut.angelic_match_sum, CMut.angelic_match_sum.
-      eapply approx_angelic_binary, approx_bind.
-      - eapply approx_bind; try (eapply approx_angelic; assumption).
+      unfold SHeapSpecM.angelic_match_sum, CHeapSpecM.angelic_match_sum.
+      apply refine_angelic_binary, refine_bind.
+      - apply refine_bind; try (apply refine_angelic; assumption).
         intros w1 r01 ι1 -> Hpc1.
-        intros v1 vc1 ->.
-        eapply approx_bind_right.
-        * eapply approx_assert_formula; try assumption. cbn.
+        intros v1 vc1 Hv1. hnf in Hv1. subst.
+        apply refine_bind.
+        * apply refine_assert_formula; try assumption. cbn.
           now rewrite <- inst_persist.
-        * intros w2 r12 ι2 -> Hpc2.
-          eapply (approx_four Hk__l); eauto.
+        * intros w2 r12 ι2 -> Hpc2 _ _ _.
+          eapply (refine_four Hk__l); cbn; eauto.
+          now rewrite inst_sub_id, ?sub_acc_trans, ?inst_subst.
           now rewrite <- inst_persist.
-      - now eapply approx_angelic.
+      - now apply refine_angelic.
       - intros w1 r01 ι1 -> Hpc1.
-        intros v1 vc1 ->.
-        eapply approx_bind_right.
-        + eapply approx_assert_formula; try assumption.
+        intros v1 vc1 Hv1. hnf in Hv1. subst.
+        apply refine_bind.
+        + apply refine_assert_formula; try assumption.
           now rewrite <- inst_persist.
-        + intros w2 r12 ι2 -> Hpc2.
-          eapply (approx_four Hk__r); eauto.
+        + intros w2 r12 ι2 -> Hpc2 _ _ _.
+          eapply (refine_four Hk__r); cbn; eauto.
+          now rewrite inst_sub_id, ?sub_acc_trans, ?inst_subst.
           now rewrite <- inst_persist.
     Qed.
 
-    Lemma approx_demonic_match_sum {AT A} `{Approx AT A} {Γ1 Γ2} x y σ τ
+    Lemma refine_demonic_match_sum {AT A} `{Refine AT A} {Γ1 Γ2} x y σ τ
       {w : World} (ι : Valuation w) (Hpc : instpc (wco w) ι) :
-      approx ι (@SMut.demonic_match_sum AT Γ1 Γ2 x y σ τ w) (@CMut.demonic_match_sum A Γ1 Γ2 σ τ).
+      ℛ ι (@SHeapSpecM.demonic_match_sum AT Γ1 Γ2 x y σ τ w) (@CHeapSpecM.demonic_match_sum A Γ1 Γ2 σ τ).
     Proof.
       intros t v ->.
       intros kl kl__c Hk__l.
       intros kr kr__c Hk__r.
-      unfold SMut.demonic_match_sum, CMut.demonic_match_sum.
-      eapply approx_demonic_binary, approx_bind.
-      - eapply approx_bind; try (eapply approx_demonic; assumption).
+      unfold SHeapSpecM.demonic_match_sum, CHeapSpecM.demonic_match_sum.
+      apply refine_demonic_binary, refine_bind.
+      - apply refine_bind; try (apply refine_demonic; assumption).
         intros w1 r01 ι1 -> Hpc1.
-        intros v1 vc1 ->.
-        eapply approx_bind_right.
-        * eapply approx_assume_formula; try assumption.
+        intros v1 vc1 Hv. hnf in Hv. subst.
+        apply refine_bind.
+        * apply refine_assume_formula; try assumption.
           now rewrite <- inst_persist.
-        * intros w2 r12 ι2 -> Hpc2.
-          eapply (approx_four Hk__l); eauto.
+        * intros w2 r12 ι2 -> Hpc2 _ _ _.
+          eapply (refine_four Hk__l); cbn; eauto.
+          now rewrite inst_sub_id, ?sub_acc_trans, ?inst_subst.
           now rewrite <- inst_persist.
-      - now eapply approx_demonic.
+      - now apply refine_demonic.
       - intros w1 r01 ι1 -> Hpc1.
-        intros v1 vc1 ->.
-        eapply approx_bind_right.
-        + eapply approx_assume_formula; try assumption.
+        intros v1 vc1 Hv. hnf in Hv. subst.
+        apply refine_bind.
+        + apply refine_assume_formula; try assumption.
           now rewrite <- inst_persist.
-        + intros w2 r12 ι2 -> Hpc2.
-          eapply (approx_four Hk__r); eauto.
+        + intros w2 r12 ι2 -> Hpc2 _ _ _.
+          eapply (refine_four Hk__r); cbn; eauto.
+          now rewrite inst_sub_id, ?sub_acc_trans, ?inst_subst.
           now rewrite <- inst_persist.
     Qed.
 
-    Lemma approx_angelic_match_prod {AT A} `{Approx AT A} {Γ1 Γ2} x y σ τ
+    Lemma refine_angelic_match_prod {AT A} `{Refine AT A} {Γ1 Γ2} x y σ τ
       {w : World} (ι : Valuation w) (Hpc : instpc (wco w) ι) :
-      approx ι (@SMut.angelic_match_prod AT Γ1 Γ2 x y σ τ w) (@CMut.angelic_match_prod A Γ1 Γ2 σ τ).
+      ℛ ι (@SHeapSpecM.angelic_match_prod AT Γ1 Γ2 x y σ τ w) (@CHeapSpecM.angelic_match_prod A Γ1 Γ2 σ τ).
     Proof.
       intros t v ->.
       intros k k__c Hk.
-      unfold SMut.angelic_match_prod, CMut.angelic_match_prod.
-      eapply approx_bind; try (eapply approx_angelic; assumption).
+      unfold SHeapSpecM.angelic_match_prod, CHeapSpecM.angelic_match_prod.
+      apply refine_bind; try (apply refine_angelic; assumption).
       intros w1 r01 ι1 -> Hpc1.
       intros v1 vc1 ->.
-      eapply approx_bind; try (eapply approx_angelic; assumption).
+      apply refine_bind; try (apply refine_angelic; assumption).
       intros w2 r12 ι2 -> Hpc2.
       intros v2 vc2 ->.
-      eapply approx_bind_right.
-      - eapply approx_assert_formula; try assumption. cbn - [Val].
+      apply refine_bind.
+      - apply refine_assert_formula; try assumption. cbn - [Val].
         change (inst_term ?t ?ι) with (inst t ι).
         rewrite (inst_persist (AT := STerm _) (A := Val _)).
         rewrite (inst_persist (AT := STerm _) (A := Val _)).
         now rewrite sub_acc_trans, inst_subst.
-      - intros w3 r23 ι3 -> Hpc3.
-        eapply (approx_four Hk); eauto.
+      - intros w3 r23 ι3 -> Hpc3 _ _ _.
+        eapply (refine_four Hk); eauto.
         + now rewrite sub_acc_trans, inst_subst.
         + rewrite <- ?inst_subst, <- subst_sub_comp.
           now rewrite <- sub_acc_trans, inst_subst, <- inst_persist.
         + now rewrite <- inst_persist.
     Qed.
 
-    Lemma approx_demonic_match_prod {AT A} `{Approx AT A} {Γ1 Γ2} x y σ τ
+    Lemma refine_demonic_match_prod {AT A} `{Refine AT A} {Γ1 Γ2} x y σ τ
       {w : World} (ι : Valuation w) (Hpc : instpc (wco w) ι) :
-      approx ι (@SMut.demonic_match_prod AT Γ1 Γ2 x y σ τ w) (@CMut.demonic_match_prod A Γ1 Γ2 σ τ).
+      ℛ ι (@SHeapSpecM.demonic_match_prod AT Γ1 Γ2 x y σ τ w) (@CHeapSpecM.demonic_match_prod A Γ1 Γ2 σ τ).
     Proof.
       intros t v ->.
       intros k k__c Hk.
-      unfold SMut.demonic_match_prod, CMut.demonic_match_prod.
-      apply approx_bind; try (eapply approx_demonic; assumption).
+      unfold SHeapSpecM.demonic_match_prod, CHeapSpecM.demonic_match_prod.
+      apply refine_bind; try (apply refine_demonic; assumption).
       intros w1 r01 ι1 -> Hpc1.
       intros v1 vc1 ->.
-      apply approx_bind; try (eapply approx_demonic; assumption).
+      apply refine_bind; try (apply refine_demonic; assumption).
       intros w2 r12 ι2 -> Hpc2.
       intros v2 vc2 ->.
-      apply approx_bind_right.
-      - apply approx_assume_formula; try assumption. cbn - [Val].
+      apply refine_bind.
+      - apply refine_assume_formula; try assumption. cbn - [Val].
         change (inst_term ?t ?ι) with (inst t ι).
         rewrite (inst_persist (AT := STerm _) (A := Val _)).
         rewrite (inst_persist (AT := STerm _) (A := Val _)).
         now rewrite sub_acc_trans, inst_subst.
-      - intros w3 r23 ι3 -> Hpc3.
-        eapply (approx_four Hk); eauto.
+      - intros w3 r23 ι3 -> Hpc3 _ _ _.
+        eapply (refine_four Hk); eauto.
         + now rewrite sub_acc_trans, inst_subst.
         + rewrite <- ?inst_subst, <- subst_sub_comp.
           now rewrite <- sub_acc_trans, inst_subst, <- inst_persist.
         + now rewrite <- inst_persist.
     Qed.
 
-    Lemma approx_angelic_match_list {AT A} `{Approx AT A} {Γ1 Γ2} xhead xtail σ
+    Lemma refine_angelic_match_list {AT A} `{Refine AT A} {Γ1 Γ2} xhead xtail σ
       {w : World} (ι : Valuation w) (Hpc : instpc (wco w) ι) :
-      approx ι (@SMut.angelic_match_list AT Γ1 Γ2 xhead xtail σ w) (@CMut.angelic_match_list A Γ1 Γ2 σ).
+      ℛ ι (@SHeapSpecM.angelic_match_list AT Γ1 Γ2 xhead xtail σ w) (@CHeapSpecM.angelic_match_list A Γ1 Γ2 σ).
     Proof.
       intros t ? ->.
       intros sknil cknil Hknil.
       intros skcons ckcons Hkcons.
-      unfold SMut.angelic_match_list, CMut.angelic_match_list.
-      apply approx_angelic_binary.
-      - apply approx_bind_right; auto.
-        apply approx_assert_formula; auto.
-      - apply approx_bind; auto.
-        apply approx_angelic; auto.
+      unfold SHeapSpecM.angelic_match_list, CHeapSpecM.angelic_match_list.
+      apply refine_angelic_binary.
+      - apply refine_bind; auto.
+        apply refine_assert_formula; auto.
+        intros ? ? ? -> ? _ _ _; auto.
+      - apply refine_bind; auto.
+        apply refine_angelic; auto.
         intros w1 ω01 ι1 -> Hpc1.
         intros thead vhead ->.
-        apply approx_bind; auto.
-        apply approx_angelic; auto.
+        apply refine_bind; auto.
+        apply refine_angelic; auto.
         intros w2 ω12 ι2 -> Hpc2.
         intros ttail vtail ->.
-        apply approx_bind_right; auto.
-        + apply approx_assert_formula; auto.
+        apply refine_bind; auto.
+        + apply refine_assert_formula; auto.
           cbn - [Val].
           change (inst_term ?t ?ι) with (inst t ι).
           rewrite (inst_persist (AT := STerm _) (A := Val _)).
           rewrite (inst_persist (AT := STerm _) (A := Val _)).
           now rewrite sub_acc_trans, inst_subst.
-        + intros w3 ω23 ι3 -> Hpc3.
+        + intros w3 ω23 ι3 -> Hpc3 _ _ _.
           apply Hkcons; wsimpl; eauto.
           rewrite <- ?inst_subst, <- subst_sub_comp.
           now rewrite <- sub_acc_trans, inst_subst, <- inst_persist.
           now rewrite <- inst_persist.
     Qed.
 
-    Lemma approx_demonic_match_list {AT A} `{Approx AT A} {Γ1 Γ2} xhead xtail σ
+    Lemma refine_demonic_match_list {AT A} `{Refine AT A} {Γ1 Γ2} xhead xtail σ
       {w : World} (ι : Valuation w) (Hpc : instpc (wco w) ι) :
-      approx ι (@SMut.demonic_match_list AT Γ1 Γ2 xhead xtail σ w) (@CMut.demonic_match_list A Γ1 Γ2 σ).
+      ℛ ι (@SHeapSpecM.demonic_match_list AT Γ1 Γ2 xhead xtail σ w) (@CHeapSpecM.demonic_match_list A Γ1 Γ2 σ).
     Proof.
       intros t ? ->.
       intros sknil cknil Hknil.
       intros skcons ckcons Hkcons.
-      unfold SMut.demonic_match_list, CMut.demonic_match_list.
-      apply approx_demonic_binary.
-      - apply approx_bind_right; auto.
-        apply approx_assume_formula; auto.
-      - apply approx_bind; auto.
-        apply approx_demonic; auto.
+      unfold SHeapSpecM.demonic_match_list, CHeapSpecM.demonic_match_list.
+      apply refine_demonic_binary.
+      - apply refine_bind; auto.
+        apply refine_assume_formula; auto.
+        intros ? ? ? -> ? _ _ _; auto.
+      - apply refine_bind; auto.
+        apply refine_demonic; auto.
         intros w1 ω01 ι1 -> Hpc1.
         intros thead vhead ->.
-        apply approx_bind; auto.
-        apply approx_demonic; auto.
+        apply refine_bind; auto.
+        apply refine_demonic; auto.
         intros w2 ω12 ι2 -> Hpc2.
         intros ttail vtail ->.
-        apply approx_bind_right; auto.
-        + apply approx_assume_formula; auto.
+        apply refine_bind; auto.
+        + apply refine_assume_formula; auto.
           cbn - [Val].
           change (inst_term ?t ?ι) with (inst t ι).
           rewrite (inst_persist (AT := STerm _) (A := Val _)).
           rewrite (inst_persist (AT := STerm _) (A := Val _)).
           now rewrite sub_acc_trans, inst_subst.
-        + intros w3 ω23 ι3 -> Hpc3.
+        + intros w3 ω23 ι3 -> Hpc3 _ _ _.
           apply Hkcons; wsimpl; eauto.
           rewrite <- ?inst_subst, <- subst_sub_comp.
           now rewrite <- sub_acc_trans, inst_subst, <- inst_persist.
           now rewrite <- inst_persist.
     Qed.
 
-    Lemma approx_angelic_match_record' {N : Set} (n : N -> 𝑺) {R AT A} `{Approx AT A} {Γ1 Γ2}
+    Lemma refine_angelic_match_record' {N : Set} (n : N -> 𝑺) {R AT A} `{Refine AT A} {Γ1 Γ2}
       {Δ : NCtx N Ty} {p : RecordPat (recordf_ty R) Δ}
       {w : World} (ι : Valuation w) (Hpc : instpc (wco w) ι) :
-      approx ι (@SMut.angelic_match_record' N n AT R Γ1 Γ2 Δ p w) (@CMut.angelic_match_record N A R Γ1 Γ2 Δ p).
+      ℛ ι (@SHeapSpecM.angelic_match_record' N n AT R Γ1 Γ2 Δ p w) (@CHeapSpecM.angelic_match_record N A R Γ1 Γ2 Δ p).
     Proof.
       intros t v ->.
       intros k k__c Hk.
-      unfold SMut.angelic_match_record', CMut.angelic_match_record.
-      eapply approx_bind; try (eapply approx_angelic_ctx; assumption).
+      unfold SHeapSpecM.angelic_match_record', CHeapSpecM.angelic_match_record.
+      apply refine_bind; try (apply refine_angelic_ctx; assumption).
       intros w1 r01 ι1 -> Hpc1.
       intros v1 vc1 ->.
-      apply approx_bind_right.
-      - apply approx_assert_formula; try assumption. cbn - [Val].
+      apply refine_bind.
+      - apply refine_assert_formula; try assumption. cbn - [Val].
         now rewrite <- inst_persist, (inst_record_pattern_match_reverse ι1 p).
-      - intros w2 r12 ι2 -> Hpc2.
-        eapply (approx_four Hk); eauto.
+      - intros w2 r12 ι2 -> Hpc2 _ _ _.
+        eapply (refine_four Hk); eauto.
         now rewrite <- inst_persist.
     Qed.
 
-    Lemma approx_angelic_match_record {N : Set} (n : N -> 𝑺) {R AT A} `{Approx AT A} {Γ1 Γ2}
+    Lemma refine_angelic_match_record {N : Set} (n : N -> 𝑺) {R AT A} `{Refine AT A} {Γ1 Γ2}
       {Δ : NCtx N Ty} {p : RecordPat (recordf_ty R) Δ}
       {w : World} (ι : Valuation w) (Hpc : instpc (wco w) ι) :
-      approx ι (@SMut.angelic_match_record N n AT R Γ1 Γ2 Δ p w) (@CMut.angelic_match_record N A R Γ1 Γ2 Δ p).
+      ℛ ι (@SHeapSpecM.angelic_match_record N n AT R Γ1 Γ2 Δ p w) (@CHeapSpecM.angelic_match_record N A R Γ1 Γ2 Δ p).
     Proof.
       intros t v ->.
       intros c c__c Hc.
-      unfold SMut.angelic_match_record.
+      unfold SHeapSpecM.angelic_match_record.
       destruct (term_get_record_spec t).
       - intros P2 Pc2 HP2.
         intros c2 cc2 Hc2.
         intros s2 sc2 Hs2.
         hnf.
-        rewrite CMut.wp_angelic_match_record.
+        rewrite CHeapSpecM.wp_angelic_match_record.
         apply Hc; wsimpl; eauto.
         hnf.
         unfold record_pattern_match_val.
         rewrite H0. rewrite recordv_unfold_fold.
         symmetry.
         apply inst_record_pattern_match.
-      - apply approx_angelic_match_record'; auto.
+      - apply refine_angelic_match_record'; auto.
     Qed.
 
-    Lemma approx_demonic_match_record' {N : Set} (n : N -> 𝑺) {R AT A} `{Approx AT A} {Γ1 Γ2}
+    Lemma refine_demonic_match_record' {N : Set} (n : N -> 𝑺) {R AT A} `{Refine AT A} {Γ1 Γ2}
       {Δ : NCtx N Ty} {p : RecordPat (recordf_ty R) Δ}
       {w : World} (ι : Valuation w) (Hpc : instpc (wco w) ι) :
-      approx ι (@SMut.demonic_match_record' N n AT R Γ1 Γ2 Δ p w) (@CMut.demonic_match_record N A R Γ1 Γ2 Δ p).
+      ℛ ι (@SHeapSpecM.demonic_match_record' N n AT R Γ1 Γ2 Δ p w) (@CHeapSpecM.demonic_match_record N A R Γ1 Γ2 Δ p).
     Proof.
       intros t v ->.
       intros k k__c Hk.
-      unfold SMut.demonic_match_record', CMut.demonic_match_record.
-      eapply approx_bind. try (eapply approx_demonic_ctx; assumption).
+      unfold SHeapSpecM.demonic_match_record', CHeapSpecM.demonic_match_record.
+      apply refine_bind. try (apply refine_demonic_ctx; assumption).
       intros w1 r01 ι1 -> Hpc1.
       intros v1 vc1 ->.
-      eapply approx_bind_right.
-      - eapply approx_assume_formula; try assumption. cbn - [Val].
+      apply refine_bind.
+      - apply refine_assume_formula; try assumption. cbn - [Val].
         now rewrite <- inst_persist, (inst_record_pattern_match_reverse ι1 p).
-      - intros w2 r12 ι2 -> Hpc2.
-        eapply (approx_four Hk); eauto.
+      - intros w2 r12 ι2 -> Hpc2 _ _ _.
+        eapply (refine_four Hk); eauto.
         now rewrite <- inst_persist.
     Qed.
 
-    Lemma approx_demonic_match_record {N : Set} (n : N -> 𝑺) {R AT A} `{Approx AT A} {Γ1 Γ2}
+    Lemma refine_demonic_match_record {N : Set} (n : N -> 𝑺) {R AT A} `{Refine AT A} {Γ1 Γ2}
       {Δ : NCtx N Ty} {p : RecordPat (recordf_ty R) Δ}
       {w : World} (ι : Valuation w) (Hpc : instpc (wco w) ι) :
-      approx ι (@SMut.demonic_match_record N n AT R Γ1 Γ2 Δ p w) (@CMut.demonic_match_record N A R Γ1 Γ2 Δ p).
+      ℛ ι (@SHeapSpecM.demonic_match_record N n AT R Γ1 Γ2 Δ p w) (@CHeapSpecM.demonic_match_record N A R Γ1 Γ2 Δ p).
     Proof.
       intros t v ->.
       intros c c__c Hc.
-      unfold SMut.demonic_match_record.
+      unfold SHeapSpecM.demonic_match_record.
       destruct (term_get_record_spec t).
       - intros P2 Pc2 HP2.
         intros c2 cc2 Hc2.
         intros s2 sc2 Hs2.
         hnf.
-        rewrite CMut.wp_demonic_match_record.
+        rewrite CHeapSpecM.wp_demonic_match_record.
         apply Hc; wsimpl; eauto.
         hnf.
         unfold record_pattern_match_val.
         rewrite H0. rewrite recordv_unfold_fold.
         change (fun Σ => @Env (N ∷ Ty) (fun τ => Term Σ (type τ)) Δ) with (fun Σ => @NamedEnv N Ty (Term Σ) Δ).
         now rewrite inst_record_pattern_match.
-      - apply approx_demonic_match_record'; auto.
+      - apply refine_demonic_match_record'; auto.
     Qed.
 
-    Lemma approx_angelic_match_tuple {N : Set} (n : N -> 𝑺) {σs AT A} `{Approx AT A} {Γ1 Γ2}
+    Lemma refine_angelic_match_tuple {N : Set} (n : N -> 𝑺) {σs AT A} `{Refine AT A} {Γ1 Γ2}
       {Δ : NCtx N Ty} {p : TuplePat σs Δ}
       {w : World} (ι : Valuation w) (Hpc : instpc (wco w) ι) :
-      approx ι (@SMut.angelic_match_tuple N n AT σs Γ1 Γ2 Δ p w) (@CMut.angelic_match_tuple N A σs Γ1 Γ2 Δ p).
+      ℛ ι (@SHeapSpecM.angelic_match_tuple N n AT σs Γ1 Γ2 Δ p w) (@CHeapSpecM.angelic_match_tuple N A σs Γ1 Γ2 Δ p).
     Proof.
       intros t v ->.
       intros k k__c Hk.
-      unfold SMut.angelic_match_tuple, CMut.angelic_match_tuple.
-      apply approx_bind; try (apply approx_angelic_ctx; assumption).
+      unfold SHeapSpecM.angelic_match_tuple, CHeapSpecM.angelic_match_tuple.
+      apply refine_bind; try (apply refine_angelic_ctx; assumption).
       intros w1 r01 ι1 -> Hpc1.
       intros v1 vc1 ->.
       change (fun Σ => @Env (N ∷ Ty) (fun τ => Term Σ (type τ)) Δ) with (fun Σ => @NamedEnv N Ty (Term Σ) Δ).
-      apply approx_bind_right.
-      - apply approx_assert_formula; try assumption. cbn - [Val].
+      apply refine_bind.
+      - apply refine_assert_formula; try assumption. cbn - [Val].
         rewrite inst_term_tuple.
         rewrite inst_tuple_pattern_match_reverse.
         rewrite <- inst_persist.
@@ -1128,25 +1235,25 @@ Module Soundness
         split; intros <-.
         + now rewrite tuple_pattern_match_env_inverse_left, envrec.of_to_env.
         + now rewrite envrec.to_of_env, tuple_pattern_match_env_inverse_right.
-      - intros w2 r12 ι2 -> Hpc2.
-        eapply (approx_four Hk); eauto.
+      - intros w2 r12 ι2 -> Hpc2 _ _ _.
+        eapply (refine_four Hk); eauto.
         now rewrite <- inst_persist.
     Qed.
 
-    Lemma approx_demonic_match_tuple {N : Set} (n : N -> 𝑺) {σs AT A} `{Approx AT A} {Γ1 Γ2}
+    Lemma refine_demonic_match_tuple {N : Set} (n : N -> 𝑺) {σs AT A} `{Refine AT A} {Γ1 Γ2}
       {Δ : NCtx N Ty} {p : TuplePat σs Δ}
       {w : World} (ι : Valuation w) (Hpc : instpc (wco w) ι) :
-      approx ι (@SMut.demonic_match_tuple N n AT σs Γ1 Γ2 Δ p w) (@CMut.demonic_match_tuple N A σs Γ1 Γ2 Δ p).
+      ℛ ι (@SHeapSpecM.demonic_match_tuple N n AT σs Γ1 Γ2 Δ p w) (@CHeapSpecM.demonic_match_tuple N A σs Γ1 Γ2 Δ p).
     Proof.
       intros t v ->.
       intros k k__c Hk.
-      unfold SMut.demonic_match_tuple, CMut.demonic_match_tuple.
-      apply approx_bind; try (apply approx_demonic_ctx; assumption).
+      unfold SHeapSpecM.demonic_match_tuple, CHeapSpecM.demonic_match_tuple.
+      apply refine_bind; try (apply refine_demonic_ctx; assumption).
       intros w1 r01 ι1 -> Hpc1.
       intros v1 vc1 ->.
       change (fun Σ => @Env (N ∷ Ty) (fun τ => Term Σ (type τ)) Δ) with (fun Σ => @NamedEnv N Ty (Term Σ) Δ).
-      apply approx_bind_right.
-      - apply approx_assume_formula; try assumption. cbn - [Val].
+      apply refine_bind.
+      - apply refine_assume_formula; try assumption. cbn - [Val].
         rewrite inst_term_tuple.
         rewrite inst_tuple_pattern_match_reverse.
         rewrite <- inst_persist.
@@ -1154,168 +1261,168 @@ Module Soundness
         split; intros <-.
         + now rewrite tuple_pattern_match_env_inverse_left, envrec.of_to_env.
         + now rewrite envrec.to_of_env, tuple_pattern_match_env_inverse_right.
-      - intros w2 r12 ι2 -> Hpc2.
-        eapply (approx_four Hk); eauto.
+      - intros w2 r12 ι2 -> Hpc2 _ _ _.
+        eapply (refine_four Hk); eauto.
         now rewrite <- inst_persist.
     Qed.
 
-    Lemma approx_angelic_match_pattern {N : Set} (n : N -> 𝑺) {σ} {Δ : NCtx N Ty}
+    Lemma refine_angelic_match_pattern {N : Set} (n : N -> 𝑺) {σ} {Δ : NCtx N Ty}
           {p : Pattern Δ σ} {Γ}
       {w : World} (ι : Valuation w) (Hpc : instpc (wco w) ι) {msg} :
-      approx ι (@SMut.angelic_match_pattern N n σ Δ p Γ w msg) (@CMut.angelic_match_pattern N σ Δ p Γ).
+      ℛ ι (@SHeapSpecM.angelic_match_pattern N n σ Δ p Γ w msg) (@CHeapSpecM.angelic_match_pattern N σ Δ p Γ).
     Proof.
       intros t v ->.
       intros k k__c Hk.
-      unfold SMut.angelic_match_pattern, CMut.angelic_match_pattern.
-      eapply approx_bind; try (eapply approx_angelic_ctx; assumption); try assumption.
+      unfold SHeapSpecM.angelic_match_pattern, CHeapSpecM.angelic_match_pattern.
+      apply refine_bind; try (apply refine_angelic_ctx; assumption); try assumption.
       intros w1 r01 ι1 -> Hpc1.
       intros ts vs ->.
       change (fun Σ => @Env (N ∷ Ty) (fun τ => Term Σ (type τ)) Δ) with (fun Σ => @NamedEnv N Ty (Term Σ) Δ).
-      eapply approx_bind_right.
-      - eapply approx_assert_formula; try assumption. cbn - [Val].
+      apply refine_bind.
+      - apply refine_assert_formula; try assumption. cbn - [Val].
         rewrite inst_pattern_match_env_reverse.
         rewrite <- inst_persist.
         split; intros <-.
         + now rewrite pattern_match_val_inverse_left.
         + now rewrite pattern_match_val_inverse_right.
-      - intros w2 r12 ι2 -> Hpc2.
-        eapply approx_pure; try assumption.
+      - intros w2 r12 ι2 -> Hpc2 _ _ _.
+        apply refine_pure; try assumption.
         now rewrite <- inst_persist.
     Qed.
 
-    Lemma approx_angelic_match_union {N : Set} (n : N -> 𝑺) {AT A} `{Approx AT A} {Γ1 Γ2 : PCtx} {U : unioni}
+    Lemma refine_angelic_match_union {N : Set} (n : N -> 𝑺) {AT A} `{Refine AT A} {Γ1 Γ2 : PCtx} {U : unioni}
       {Δ : unionk U -> NCtx N Ty} {p : forall K : unionk U, Pattern (Δ K) (unionk_ty U K)}
       {w : World} (ι : Valuation w) (Hpc : instpc (wco w) ι) :
-      approx ι (@SMut.angelic_match_union N n AT Γ1 Γ2 U Δ p w) (@CMut.angelic_match_union N A Γ1 Γ2 U Δ p).
+      ℛ ι (@SHeapSpecM.angelic_match_union N n AT Γ1 Γ2 U Δ p w) (@CHeapSpecM.angelic_match_union N A Γ1 Γ2 U Δ p).
     Proof.
       intros t v ->.
       intros k k__c Hk.
-      unfold SMut.angelic_match_union, CMut.angelic_match_union.
-      apply approx_bind; try (apply approx_angelic_finite; assumption).
+      unfold SHeapSpecM.angelic_match_union, CHeapSpecM.angelic_match_union.
+      apply refine_bind; try (apply refine_angelic_finite; assumption).
       intros w1 r01 ι1 -> Hpc1.
       intros v1 vc1 ->.
-      apply approx_bind; try (apply approx_angelic; assumption).
+      apply refine_bind; try (apply refine_angelic; assumption).
       intros w2 r12 ι2 -> Hpc2.
       intros v2 vc2 ->.
-      eapply approx_bind_right.
-      - eapply approx_assert_formula; try assumption. cbn - [Val].
+      apply refine_bind.
+      - apply refine_assert_formula; try assumption. cbn - [Val].
         change (inst v1 _) with v1.
         change (inst_term ?t ?ι) with (inst t ι).
         rewrite (inst_persist (AT := STerm _) (A := Val _)).
         now rewrite sub_acc_trans, inst_subst.
-      - intros w3 r23 ι3 -> Hpc3.
-        eapply approx_bind.
-        + eapply approx_angelic_match_pattern; try assumption.
+      - intros w3 r23 ι3 -> Hpc3 _ _ _.
+        apply refine_bind.
+        + apply refine_angelic_match_pattern; try assumption.
           now rewrite <- inst_persist.
         + change (inst v1 _) with v1.
           specialize (Hk v1).
-          eapply (approx_four Hk).
+          eapply (refine_four Hk).
           now rewrite ?sub_acc_trans, ?inst_subst.
     Qed.
 
-    Lemma approx_demonic_match_pattern {N : Set} (n : N -> 𝑺) {σ} {Δ : NCtx N Ty}
+    Lemma refine_demonic_match_pattern {N : Set} (n : N -> 𝑺) {σ} {Δ : NCtx N Ty}
           {p : Pattern Δ σ} {Γ}
       {w : World} (ι : Valuation w) (Hpc : instpc (wco w) ι) :
-      approx ι (@SMut.demonic_match_pattern N n σ Δ p Γ w) (@CMut.demonic_match_pattern N σ Δ p Γ).
+      ℛ ι (@SHeapSpecM.demonic_match_pattern N n σ Δ p Γ w) (@CHeapSpecM.demonic_match_pattern N σ Δ p Γ).
     Proof.
       intros t v ->.
       intros k k__c Hk.
-      unfold SMut.demonic_match_pattern, CMut.demonic_match_pattern.
-      eapply approx_bind; try (eapply approx_demonic_ctx; assumption); try assumption.
+      unfold SHeapSpecM.demonic_match_pattern, CHeapSpecM.demonic_match_pattern.
+      apply refine_bind; try (apply refine_demonic_ctx; assumption); try assumption.
       intros w1 r01 ι1 -> Hpc1.
       intros ts vs ->.
       change (fun Σ => @Env (N ∷ Ty) (fun τ => Term Σ (type τ)) Δ) with (fun Σ => @NamedEnv N Ty (Term Σ) Δ).
-      eapply approx_bind_right.
-      - eapply approx_assume_formula; try assumption. cbn - [Val].
+      apply refine_bind.
+      - apply refine_assume_formula; try assumption. cbn - [Val].
         rewrite inst_pattern_match_env_reverse.
         rewrite <- inst_persist.
         split; intros <-.
         + now rewrite pattern_match_val_inverse_left.
         + now rewrite pattern_match_val_inverse_right.
-      - intros w2 r12 ι2 -> Hpc2.
-        eapply approx_pure; try assumption.
+      - intros w2 r12 ι2 -> Hpc2 _ _ _.
+        apply refine_pure; try assumption.
         now rewrite <- inst_persist.
     Qed.
 
-    Lemma approx_demonic_match_union {N : Set} (n : N -> 𝑺) {AT A} `{Approx AT A} {Γ1 Γ2 : PCtx} {U : unioni}
+    Lemma refine_demonic_match_union {N : Set} (n : N -> 𝑺) {AT A} `{Refine AT A} {Γ1 Γ2 : PCtx} {U : unioni}
       {Δ : unionk U -> NCtx N Ty} {p : forall K : unionk U, Pattern (Δ K) (unionk_ty U K)}
       {w : World} (ι : Valuation w) (Hpc : instpc (wco w) ι) :
-      approx ι (@SMut.demonic_match_union N n AT Γ1 Γ2 U Δ p w) (@CMut.demonic_match_union N A Γ1 Γ2 U Δ p).
+      ℛ ι (@SHeapSpecM.demonic_match_union N n AT Γ1 Γ2 U Δ p w) (@CHeapSpecM.demonic_match_union N A Γ1 Γ2 U Δ p).
     Proof.
       intros t v ->.
       intros k k__c Hk.
-      unfold SMut.demonic_match_union, CMut.demonic_match_union.
-      eapply approx_bind; try (eapply approx_demonic_finite; assumption).
+      unfold SHeapSpecM.demonic_match_union, CHeapSpecM.demonic_match_union.
+      apply refine_bind; try (apply refine_demonic_finite; assumption).
       intros w1 r01 ι1 -> Hpc1.
       intros v1 vc1 ->.
-      eapply approx_bind; try (eapply approx_demonic; assumption).
+      apply refine_bind; try (apply refine_demonic; assumption).
       intros w2 r12 ι2 -> Hpc2.
       intros v2 vc2 ->.
-      eapply approx_bind_right.
-      - eapply approx_assume_formula; try assumption. cbn - [Val].
+      apply refine_bind.
+      - apply refine_assume_formula; try assumption. cbn - [Val].
         change (inst v1 _) with v1.
         change (inst_term ?t ?ι) with (inst t ι).
         rewrite (inst_persist (AT := STerm _) (A := Val _)).
         now rewrite sub_acc_trans, inst_subst.
-      - intros w3 r23 ι3 -> Hpc3.
-        eapply approx_bind.
-        + eapply approx_demonic_match_pattern; try assumption.
+      - intros w3 r23 ι3 -> Hpc3 _ _ _.
+        apply refine_bind.
+        + apply refine_demonic_match_pattern; try assumption.
           now rewrite <- inst_persist.
         + change (inst v1 _) with v1.
           specialize (Hk v1).
-          eapply (approx_four Hk).
+          eapply (refine_four Hk).
           now rewrite ?sub_acc_trans, ?inst_subst.
     Qed.
 
-    Lemma approx_demonic_match_bvec' {AT A} `{Approx AT A} {n : nat} {Γ1 Γ2 : PCtx}
+    Lemma refine_demonic_match_bvec' {AT A} `{Refine AT A} {n : nat} {Γ1 Γ2 : PCtx}
       {w : World} (ι : Valuation w) (Hpc : instpc (wco w) ι) :
-      approx ι (@SMut.demonic_match_bvec' AT n Γ1 Γ2 w) (@CMut.demonic_match_bvec A n Γ1 Γ2).
+      ℛ ι (@SHeapSpecM.demonic_match_bvec' AT n Γ1 Γ2 w) (@CHeapSpecM.demonic_match_bvec A n Γ1 Γ2).
     Proof.
       intros t v ->.
       intros ks kc Hk.
-      unfold SMut.demonic_match_bvec', CMut.demonic_match_bvec.
-      apply approx_bind.
-      apply approx_demonic_finite; auto.
+      unfold SHeapSpecM.demonic_match_bvec', CHeapSpecM.demonic_match_bvec.
+      apply refine_bind.
+      apply refine_demonic_finite; auto.
       intros w1 ω01 ι1 -> Hpc1.
-      intros EK1 EK2 ->. unfold CMut.bind_right.
-      apply approx_bind.
-      apply approx_assume_formula; cbn; wsimpl; auto.
+      intros EK1 EK2 ->. unfold CHeapSpecM.bind_right.
+      apply refine_bind.
+      apply refine_assume_formula; cbn; wsimpl; auto.
       now rewrite <- inst_persist.
       intros w2 ω12 ι2 -> Hpc2.
       intros _ _ _.
-      eapply Hk; wsimpl; auto.
+      apply Hk; wsimpl; auto.
     Qed.
 
-    Lemma approx_demonic_match_bvec {AT A} `{Approx AT A} {n : nat} {Γ1 Γ2 : PCtx}
+    Lemma refine_demonic_match_bvec {AT A} `{Refine AT A} {n : nat} {Γ1 Γ2 : PCtx}
       {w : World} (ι : Valuation w) (Hpc : instpc (wco w) ι) :
-      approx ι (@SMut.demonic_match_bvec AT n Γ1 Γ2 w) (@CMut.demonic_match_bvec A n Γ1 Γ2).
+      ℛ ι (@SHeapSpecM.demonic_match_bvec AT n Γ1 Γ2 w) (@CHeapSpecM.demonic_match_bvec A n Γ1 Γ2).
     Proof.
       intros t v ->.
       intros c c__c Hc.
-      unfold SMut.demonic_match_bvec.
+      unfold SHeapSpecM.demonic_match_bvec.
       destruct (term_get_val_spec t).
       - intros P2 Pc2 HP2.
         intros c2 cc2 Hc2.
         intros s2 sc2 Hs2.
         hnf.
-        rewrite CMut.wp_demonic_match_bvec.
+        rewrite CHeapSpecM.wp_demonic_match_bvec.
         apply Hc; wsimpl; eauto.
-      - apply approx_demonic_match_bvec'; auto.
+      - apply refine_demonic_match_bvec'; auto.
     Qed.
 
   End PatternMatching.
 
   Section State.
 
-    Lemma approx_pushpop {AT A} `{Approx AT A} {Γ1 Γ2 x σ} {w0 : World} (ι0 : Valuation w0)
+    Lemma refine_pushpop {AT A} `{Refine AT A} {Γ1 Γ2 x σ} {w0 : World} (ι0 : Valuation w0)
           (Hpc : instpc (wco w0) ι0) :
-      approx ι0 (@SMut.pushpop AT Γ1 Γ2 x σ w0) (@CMut.pushpop A Γ1 Γ2 x σ).
+      ℛ ι0 (@SHeapSpecM.pushpop AT Γ1 Γ2 x σ w0) (@CHeapSpecM.pushpop A Γ1 Γ2 x σ).
     Proof.
       intros t v ->.
       intros ms mc Hm.
       intros POST__s POST__c HPOST.
       intros δs0 δc0 -> hs0 hc0 Hh0.
-      unfold SMut.pushpop, CMut.pushpop.
+      unfold SHeapSpecM.pushpop, CHeapSpecM.pushpop.
       apply Hm; eauto.
       intros w1 ω01 ι1 -> Hpc1.
       intros a1 a Ha.
@@ -1324,15 +1431,15 @@ Module Soundness
       now destruct (env.snocView δs1).
     Qed.
 
-    Lemma approx_pushspops {AT A} `{Approx AT A} {Γ1 Γ2 Δ} {w0 : World} (ι0 : Valuation w0)
+    Lemma refine_pushspops {AT A} `{Refine AT A} {Γ1 Γ2 Δ} {w0 : World} (ι0 : Valuation w0)
           (Hpc : instpc (wco w0) ι0) :
-      approx ι0 (@SMut.pushspops AT Γ1 Γ2 Δ w0) (@CMut.pushspops A Γ1 Γ2 Δ).
+      ℛ ι0 (@SHeapSpecM.pushspops AT Γ1 Γ2 Δ w0) (@CHeapSpecM.pushspops A Γ1 Γ2 Δ).
     Proof.
       intros δΔ ? ->.
       intros ms mc Hm.
       intros POST__s POST__c HPOST.
       intros δs0 δc0 -> hs0 hc0 Hh0.
-      unfold SMut.pushspops, CMut.pushspops.
+      unfold SHeapSpecM.pushspops, CHeapSpecM.pushspops.
       apply Hm; auto.
       - intros w1 ω01 ι1 -> Hpc1.
         intros a1 a Ha.
@@ -1350,51 +1457,51 @@ Module Soundness
         reflexivity.
     Qed.
 
-    Lemma approx_get_local {Γ}
+    Lemma refine_get_local {Γ}
       {w0 : World} (ι0 : Valuation w0) (Hpc : instpc (wco w0) ι0) :
-      approx ι0 (@SMut.get_local Γ w0) (@CMut.get_local Γ).
+      ℛ ι0 (@SHeapSpecM.get_local Γ w0) (@CHeapSpecM.get_local Γ).
     Proof.
       intros POST__s POST__c HPOST.
       intros δs0 δc0 Hδ hs0 hc0 Hh0.
-      unfold SMut.get_local, CMut.get_local.
+      unfold SHeapSpecM.get_local, CHeapSpecM.get_local.
       apply HPOST; wsimpl; auto.
     Qed.
 
-    Lemma approx_put_local {Γ1 Γ2}
+    Lemma refine_put_local {Γ1 Γ2}
       {w0 : World} (ι0 : Valuation w0) (Hpc : instpc (wco w0) ι0) :
-      approx ι0 (@SMut.put_local Γ1 Γ2 w0) (@CMut.put_local Γ1 Γ2).
+      ℛ ι0 (@SHeapSpecM.put_local Γ1 Γ2 w0) (@CHeapSpecM.put_local Γ1 Γ2).
     Proof.
       intros δs2 δc2 Hδ2.
       intros POST__s POST__c HPOST.
       intros δs0 δc0 Hδ hs0 hc0 Hh0.
-      unfold SMut.put_local, CMut.put_local.
+      unfold SHeapSpecM.put_local, CHeapSpecM.put_local.
       apply HPOST; wsimpl; auto.
     Qed.
 
-    Lemma approx_get_heap {Γ}
+    Lemma refine_get_heap {Γ}
       {w0 : World} (ι0 : Valuation w0) (Hpc : instpc (wco w0) ι0) :
-      approx ι0 (@SMut.get_heap Γ w0) (@CMut.get_heap Γ).
+      ℛ ι0 (@SHeapSpecM.get_heap Γ w0) (@CHeapSpecM.get_heap Γ).
     Proof.
       intros POST__s POST__c HPOST.
       intros δs0 δc0 Hδ hs0 hc0 Hh0.
-      unfold SMut.get_heap, CMut.get_heap.
+      unfold SHeapSpecM.get_heap, CHeapSpecM.get_heap.
       apply HPOST; wsimpl; auto.
     Qed.
 
-    Lemma approx_put_heap {Γ}
+    Lemma refine_put_heap {Γ}
       {w0 : World} (ι0 : Valuation w0) (Hpc : instpc (wco w0) ι0) :
-      approx ι0 (@SMut.put_heap Γ w0) (@CMut.put_heap Γ).
+      ℛ ι0 (@SHeapSpecM.put_heap Γ w0) (@CHeapSpecM.put_heap Γ).
     Proof.
       intros hs hc Hh.
       intros POST__s POST__c HPOST.
       intros δs0 δc0 Hδ hs0 hc0 Hh0.
-      unfold SMut.put_heap, CMut.put_heap.
+      unfold SHeapSpecM.put_heap, CHeapSpecM.put_heap.
       apply HPOST; wsimpl; auto.
     Qed.
 
-    Lemma approx_eval_exp {Γ σ} (e : Exp Γ σ)
+    Lemma refine_eval_exp {Γ σ} (e : Exp Γ σ)
       {w0 : World} (ι0 : Valuation w0) (Hpc : instpc (wco w0) ι0) :
-      approx ι0 (@SMut.eval_exp Γ σ e w0) (@CMut.eval_exp Γ σ e).
+      ℛ ι0 (@SHeapSpecM.eval_exp Γ σ e w0) (@CHeapSpecM.eval_exp Γ σ e).
     Proof.
       intros POST__s POST__c HPOST.
       intros δs0 δc0 -> hs0 hc0 Hh.
@@ -1402,9 +1509,9 @@ Module Soundness
       hnf. now rewrite peval_sound, eval_exp_inst.
     Qed.
 
-    Lemma approx_eval_exps {Γ Δ} (es : NamedEnv (Exp Γ) Δ) {w0 : World} (ι0 : Valuation w0)
+    Lemma refine_eval_exps {Γ Δ} (es : NamedEnv (Exp Γ) Δ) {w0 : World} (ι0 : Valuation w0)
           (Hpc : instpc (wco w0) ι0) :
-      approx ι0 (@SMut.eval_exps Γ Δ es w0) (@CMut.eval_exps Γ Δ es).
+      ℛ ι0 (@SHeapSpecM.eval_exps Γ Δ es w0) (@CHeapSpecM.eval_exps Γ Δ es).
     Proof.
       intros POST__s POST__c HPOST.
       intros δs0 δc0 -> hs0 hc0 Hh.
@@ -1414,39 +1521,39 @@ Module Soundness
       now rewrite peval_sound, <- eval_exp_inst.
     Qed.
 
-    Lemma approx_assign {Γ x σ} {xIn : x∷σ ∈ Γ}
+    Lemma refine_assign {Γ x σ} {xIn : x∷σ ∈ Γ}
       {w0 : World} (ι0 : Valuation w0) (Hpc : instpc (wco w0) ι0) :
-      approx ι0 (@SMut.assign Γ x σ xIn w0) (@CMut.assign Γ x σ xIn).
+      ℛ ι0 (@SHeapSpecM.assign Γ x σ xIn w0) (@CHeapSpecM.assign Γ x σ xIn).
     Proof.
       intros t v ->.
       intros POST__s POST__c HPOST.
       intros δs0 δc0 -> hs0 hc0 Hh.
-      unfold SMut.assign, CMut.assign.
+      unfold SHeapSpecM.assign, CHeapSpecM.assign.
       apply HPOST; wsimpl; eauto.
       hnf. unfold inst, inst_store, inst_env.
       now rewrite env.map_update.
     Qed.
 
   End State.
-  Local Hint Resolve approx_eval_exp : core.
-  Local Hint Resolve approx_eval_exps : core.
-  Local Hint Resolve approx_pushpop : core.
-  Local Hint Resolve approx_pushspops : core.
-  Local Hint Resolve approx_debug : core.
+  Local Hint Resolve refine_eval_exp : core.
+  Local Hint Resolve refine_eval_exps : core.
+  Local Hint Resolve refine_pushpop : core.
+  Local Hint Resolve refine_pushspops : core.
+  Local Hint Resolve refine_debug : core.
 
-  Local Hint Resolve approx_demonic : core.
-  Local Hint Resolve approx_bind : core.
-  Local Hint Resolve approx_angelic_ctx : core.
-  Local Hint Resolve approx_bind_right : core.
+  Local Hint Resolve refine_demonic : core.
+  Local Hint Resolve refine_bind : core.
+  Local Hint Resolve refine_angelic_ctx : core.
+  (* Local Hint Resolve refine_bind_right : core. *)
 
-  Lemma approx_produce_chunk {Γ} {w0 : World} (ι0 : Valuation w0)
+  Lemma refine_produce_chunk {Γ} {w0 : World} (ι0 : Valuation w0)
     (Hpc0 : instpc (wco w0) ι0) :
-    approx ι0 (@SMut.produce_chunk Γ w0) (CMut.produce_chunk).
+    ℛ ι0 (@SHeapSpecM.produce_chunk Γ w0) (CHeapSpecM.produce_chunk).
   Proof.
     intros cs cc ->.
     intros POST__s POST__c HPOST.
     intros δs δc -> hs hc ->.
-    unfold SMut.produce_chunk, CMut.produce_chunk.
+    unfold SHeapSpecM.produce_chunk, CHeapSpecM.produce_chunk.
     apply HPOST; cbn; rewrite ?inst_sub_id; auto.
     hnf. cbn. now rewrite peval_chunk_sound.
   Qed.
@@ -1467,32 +1574,32 @@ Module Soundness
     apply (@inst_env_cat (𝑺 ∷ Ty) (fun Σ b => Term Σ (type b))).
   Qed.
 
-  Lemma approx_produce {Γ Σ0 pc0} (asn : Assertion Σ0) :
+  Lemma refine_produce {Γ Σ0 pc0} (asn : Assertion Σ0) :
     let w0 := @MkWorld Σ0 pc0 in
     forall
       (ι0 : Valuation w0)
       (Hpc0 : instpc (wco w0) ι0),
-      approx ι0 (@SMut.produce Γ w0 asn) (CMut.produce ι0 asn).
+      ℛ ι0 (@SHeapSpecM.produce Γ w0 asn) (CHeapSpecM.produce ι0 asn).
   Proof.
     induction asn; intros w0 * Hpc; cbn - [wctx Val].
-    - now apply approx_box_assume_formula.
+    - now apply refine_box_assume_formula.
     - intros w1 ω01 ι1 -> Hpc1.
       rewrite <- inst_persist.
-      now apply approx_produce_chunk.
+      now apply refine_produce_chunk.
     - intros w1 ω01 ι1 -> Hpc1.
       rewrite <- inst_persist.
-      now apply approx_produce_chunk.
+      now apply refine_produce_chunk.
     - intros w1 ω01 ι1 -> Hpc1.
       rewrite <- inst_persist.
-      apply approx_demonic_match_bool; eauto.
+      apply refine_demonic_match_bool; eauto.
     - intros w1 ω01 ι1 -> Hpc1.
       rewrite <- inst_persist.
-      apply approx_demonic_match_enum; auto.
+      apply refine_demonic_match_enum; auto.
       intros EK1 EK2 HEK. hnf in HEK. subst EK2.
       eauto.
     - intros w1 ω01 ι1 -> Hpc1.
       rewrite <- inst_persist.
-      apply approx_demonic_match_sum; auto.
+      apply refine_demonic_match_sum; auto.
       + intros w2 ω12 ι2 -> Hpc2.
         intros t v ->.
         apply IHasn1; cbn - [inst sub_wk1]; wsimpl; auto.
@@ -1501,21 +1608,21 @@ Module Soundness
         apply IHasn2; cbn - [inst sub_wk1]; wsimpl; auto.
     - intros w1 ω01 ι1 -> Hpc1.
       rewrite <- inst_persist.
-      apply approx_demonic_match_list; auto.
-      eapply approx_four; eauto.
+      apply refine_demonic_match_list; auto.
+      eapply refine_four; eauto.
       intros w2 ω12 ι2 -> Hpc2.
       intros thead vhead ->.
       intros ttail vtail ->.
       apply IHasn2; cbn - [inst sub_wk1]; wsimpl; auto.
     - intros w1 ω01 ι1 -> Hpc1.
       rewrite <- inst_persist.
-      apply approx_demonic_match_prod; auto.
+      apply refine_demonic_match_prod; auto.
       intros w2 ω12 ι2 -> Hpc2.
       intros t1 v1 -> t2 v2 ->.
       apply IHasn; cbn - [inst sub_wk1]; wsimpl; auto.
     - intros w1 ω01 ι1 -> Hpc1.
       rewrite <- inst_persist.
-      apply approx_demonic_match_tuple; auto.
+      apply refine_demonic_match_tuple; auto.
       intros w2 ω12 ι2 -> Hpc2.
       intros ts vs ->.
       apply IHasn; cbn - [Sub inst sub_wk1 sub_id sub_cat_left]; wsimpl; auto.
@@ -1532,7 +1639,7 @@ Module Soundness
       now rewrite inst_sub_cat, inst_subst.
     - intros w1 ω01 ι1 -> Hpc1.
       rewrite <- inst_persist.
-      apply approx_demonic_match_record; auto.
+      apply refine_demonic_match_record; auto.
       intros w2 ω12 ι2 -> Hpc2.
       intros ts vs ->.
       apply IHasn; cbn - [Sub inst sub_wk1 sub_id sub_cat_left]; wsimpl; auto.
@@ -1549,7 +1656,7 @@ Module Soundness
       now rewrite inst_sub_cat, inst_subst.
     - intros w1 ω01 ι1 -> Hpc1.
       rewrite <- inst_persist.
-      apply approx_demonic_match_union; auto.
+      apply refine_demonic_match_union; auto.
       intros UK.
       intros w2 ω12 ι2 -> Hpc2.
       intros ts vs ->.
@@ -1566,28 +1673,31 @@ Module Soundness
       }
       now rewrite inst_sub_cat, inst_subst.
     - intros w1 ω01 ι1 -> Hpc1.
-      apply approx_bind_right; eauto.
-      apply IHasn1; eauto.
+      apply refine_bind; eauto.
+      apply IHasn1; auto.
+      intros ? ? ? -> ? _ _ _.
+      apply IHasn2; auto.
+      rewrite ?inst_sub_snoc, ?sub_acc_trans, ?inst_subst, ?inst_sub_wk1; eauto.
     - intros w1 ω01 ι1 -> Hpc1.
-      apply approx_demonic_binary;
+      apply refine_demonic_binary;
         try apply IHasn1; try apply IHasn2;
         cbn - [inst sub_wk1];
         rewrite ?inst_sub_snoc, ?sub_acc_trans, ?inst_subst, ?inst_sub_wk1; eauto.
     - intros w1 ω01 ι1 -> Hpc1.
-      apply approx_bind.
-      apply approx_demonic; auto.
+      apply refine_bind.
+      apply refine_demonic; auto.
       intros w2 ω02 ι2 -> Hpc2. intros t v ->.
       apply IHasn; cbn - [inst sub_wk1];
         rewrite ?inst_sub_snoc, ?sub_acc_trans, ?inst_subst, ?inst_sub_wk1; eauto.
     - intros w1 ω01 ι1 -> Hpc1.
-      apply approx_debug; auto.
-      apply approx_pure; auto.
+      apply refine_debug; auto.
+      apply refine_pure; auto.
   Qed.
 
   Lemma try_consume_chunk_exact_spec {Σ} (h : SHeap Σ) (c : Chunk Σ) :
     option.wlp
       (fun h' => List.In (c , h') (heap_extractions h))
-      (SMut.try_consume_chunk_exact h c).
+      (SHeapSpecM.try_consume_chunk_exact h c).
   Proof.
     induction h as [|c' h].
     - now constructor.
@@ -1629,10 +1739,10 @@ Module Soundness
            List.In
              (inst (chunk_user p (eq_rect_r (fun c : Ctx Ty => Env (Term Σ) c) (tsI ►► tsO) prec)) ι, inst h' ι)
              (heap_extractions (inst h ι)))
-      (SMut.find_chunk_user_precise prec tsI tsO h).
+      (SHeapSpecM.find_chunk_user_precise prec tsI tsO h).
   Proof.
-    induction h as [|c h]; [now constructor|]. cbn [SMut.find_chunk_user_precise].
-    destruct SMut.match_chunk_user_precise as [eqs|] eqn:?.
+    induction h as [|c h]; [now constructor|]. cbn [SHeapSpecM.find_chunk_user_precise].
+    destruct SHeapSpecM.match_chunk_user_precise as [eqs|] eqn:?.
     - clear IHh. constructor. intros ι Heqs. left.
       destruct c; try discriminate Heqo. cbn in *.
       destruct (eq_dec p p0); cbn in Heqo; try discriminate Heqo. destruct e.
@@ -1661,10 +1771,10 @@ Module Soundness
            List.In
              (inst (chunk_ptsreg r t) ι, inst h' ι)
              (heap_extractions (inst h ι)))
-      (SMut.find_chunk_ptsreg_precise r t h).
+      (SHeapSpecM.find_chunk_ptsreg_precise r t h).
   Proof.
-    induction h; cbn [SMut.find_chunk_ptsreg_precise]; [now constructor|].
-    destruct SMut.match_chunk_ptsreg_precise eqn:?.
+    induction h; cbn [SHeapSpecM.find_chunk_ptsreg_precise]; [now constructor|].
+    destruct SHeapSpecM.match_chunk_ptsreg_precise eqn:?.
     - constructor. intros ι. rewrite inst_pathcondition_cons. intros [Hf Hpc].
       clear IHh. destruct a; cbn in Heqo; try discriminate Heqo.
       destruct (eq_dec_het r r0); try discriminate Heqo.
@@ -1679,24 +1789,25 @@ Module Soundness
       eexists (c', inst h' ι); auto.
   Qed.
 
-  Lemma approx_consume_chunk {Γ} {w0 : World} (ι0 : Valuation w0)
+  Lemma refine_consume_chunk {Γ} {w0 : World} (ι0 : Valuation w0)
     (Hpc0 : instpc (wco w0) ι0) :
-    approx ι0 (@SMut.consume_chunk Γ w0) (CMut.consume_chunk).
+    ℛ ι0 (@SHeapSpecM.consume_chunk Γ w0) (CHeapSpecM.consume_chunk).
   Proof.
     intros cs cc ->.
-    unfold SMut.consume_chunk, CMut.consume_chunk.
-    apply approx_bind.
-    apply approx_get_heap; auto.
+    unfold SHeapSpecM.consume_chunk, CHeapSpecM.consume_chunk.
+    apply refine_bind.
+    apply refine_get_heap; auto.
     intros w1 ω01 ι1 -> Hpc1.
     intros hs hc ->.
     remember (peval_chunk (persist cs ω01)) as c1.
     destruct (try_consume_chunk_exact_spec hs c1) as [h' HIn|].
     { intros POST__s POST__c HPOST.
       intros δs δc -> hs' hc' ->.
-      unfold approx, ApproxPath. intros Hwp.
-      cbv [SMut.put_heap CMut.bind CMut.put_heap CMut.bind_right CMut.assert_formula
-                         T CMut.angelic_list CMut.dijkstra].
-      rewrite CDijk.wp_angelic_list.
+      unfold ℛ, RefineProp. intros Hwp.
+      cbv [CHeapSpecM.assert_formula CHeapSpecM.assert_eq_chunk CHeapSpecM.bind
+           SHeapSpecM.put_heap CHeapSpecM.put_heap CHeapSpecM.bind_right T
+           CHeapSpecM.angelic_list CHeapSpecM.lift_purem ].
+      rewrite CPureSpecM.wp_angelic_list.
       change (SHeap w1) in h'.
       exists (inst c1 ι1, inst h' ι1).
       split.
@@ -1704,18 +1815,19 @@ Module Soundness
         rewrite heap_extractions_map, List.in_map_iff.
         + exists (c1 , h'). split. reflexivity. assumption.
         + eauto using inst_is_duplicable.
-      - hnf. subst. rewrite peval_chunk_sound, inst_persist.
+      - rewrite CPureSpecM.wp_assert_eq_chunk. subst.
+        rewrite peval_chunk_sound, inst_persist.
         split; auto. revert Hwp. apply HPOST; wsimpl; auto.
     }
-    destruct (SMut.try_consume_chunk_precise hs c1) as [[h' eqs]|] eqn:?.
+    destruct (SHeapSpecM.try_consume_chunk_precise hs c1) as [[h' eqs]|] eqn:?.
     { intros POST__s POST__c HPOST.
       intros δs δc -> hs' hc' ->.
-      unfold approx, ApproxPath.
-      cbv [SMut.put_heap SMut.bind_right T]. cbn. intros Hwp.
-      eapply (approx_assert_formulas Hpc1 eqs) in Hwp; eauto. destruct Hwp as [Heqs HPOST1].
-      cbv [CMut.bind CMut.put_heap CMut.bind_right CMut.assert_formula
-           T CMut.angelic_list CMut.dijkstra].
-      rewrite CDijk.wp_angelic_list.
+      unfold ℛ, RefineProp.
+      cbv [SHeapSpecM.put_heap SHeapSpecM.bind_right T]. cbn. intros Hwp.
+      eapply (refine_assert_formulas Hpc1 eqs) in Hwp; eauto. destruct Hwp as [Heqs HPOST1].
+      cbv [CHeapSpecM.bind CHeapSpecM.put_heap CHeapSpecM.bind_right CHeapSpecM.assert_formula
+           T CHeapSpecM.angelic_list CHeapSpecM.lift_purem].
+      rewrite CPureSpecM.wp_angelic_list.
       destruct c1; cbn in Heqo; try discriminate Heqo; cbn.
       - destruct (𝑯_precise p) as [[ΔI ΔO prec]|]; try discriminate Heqo.
         remember (eq_rect (𝑯_Ty p) (Env (Term w1)) ts (ΔI ▻▻ ΔO) prec) as ts'.
@@ -1726,37 +1838,39 @@ Module Soundness
         rewrite rew_opp_l in HIn. rewrite Heqc1 in HIn.
         rewrite peval_chunk_sound in HIn.
         eexists; split; eauto. clear HIn.
-        hnf. split; auto. now rewrite <- inst_persist.
+        hnf. rewrite CPureSpecM.wp_assert_eq_chunk.
+        split; auto. now rewrite <- inst_persist.
       - destruct (find_chunk_ptsreg_precise_spec r t hs) as [[h'' eqs''] HIn|];
           inversion Heqo; subst; clear Heqo.
         specialize (HIn ι1 Heqs). rewrite Heqc1 in HIn.
         rewrite peval_chunk_sound in HIn.
         eexists; split; eauto. clear HIn.
-        hnf. split; auto. now rewrite <- inst_persist.
+        hnf. rewrite CPureSpecM.wp_assert_eq_chunk.
+        split; auto. now rewrite <- inst_persist.
     }
     { intros POST__s POST__c HPOST.
       intros δs δc ? hs' hc' ? [].
     }
   Qed.
 
-  Lemma approx_consume_chunk_angelic {Γ} {w0 : World} (ι0 : Valuation w0)
+  Lemma refine_consume_chunk_angelic {Γ} {w0 : World} (ι0 : Valuation w0)
     (Hpc0 : instpc (wco w0) ι0) :
-    approx ι0 (@SMut.consume_chunk_angelic Γ w0) (CMut.consume_chunk).
+    ℛ ι0 (@SHeapSpecM.consume_chunk_angelic Γ w0) (CHeapSpecM.consume_chunk).
   Proof.
     intros cs cc ->.
-    unfold SMut.consume_chunk_angelic, CMut.consume_chunk.
-    apply approx_bind.
-    apply approx_get_heap; auto.
+    unfold SHeapSpecM.consume_chunk_angelic, CHeapSpecM.consume_chunk.
+    apply refine_bind.
+    apply refine_get_heap; auto.
     intros w1 ω01 ι1 -> Hpc1.
     intros hs hc ->.
     remember (peval_chunk (persist cs ω01)) as c1.
     destruct (try_consume_chunk_exact_spec hs c1) as [h' HIn|].
     { intros POST__s POST__c HPOST.
       intros δs δc -> hs' hc' ->.
-      unfold approx, ApproxPath. intros Hwp.
-      cbv [SMut.put_heap CMut.bind CMut.put_heap CMut.bind_right CMut.assert_formula
-                         T CMut.angelic_list CMut.dijkstra].
-      rewrite CDijk.wp_angelic_list.
+      unfold ℛ, RefineProp. intros Hwp.
+      cbv [SHeapSpecM.put_heap CHeapSpecM.bind CHeapSpecM.put_heap CHeapSpecM.bind_right CHeapSpecM.assert_formula
+                         T CHeapSpecM.angelic_list CHeapSpecM.lift_purem].
+      rewrite CPureSpecM.wp_angelic_list.
       change (SHeap w1) in h'.
       exists (inst c1 ι1, inst h' ι1).
       split.
@@ -1765,17 +1879,18 @@ Module Soundness
         + exists (c1 , h'). split. reflexivity. assumption.
         + eauto using inst_is_duplicable.
       - hnf. subst. rewrite peval_chunk_sound, inst_persist.
+        rewrite CPureSpecM.wp_assert_eq_chunk.
         split; auto. revert Hwp. apply HPOST; wsimpl; auto.
     }
-    destruct (SMut.try_consume_chunk_precise hs c1) as [[h' eqs]|] eqn:?.
+    destruct (SHeapSpecM.try_consume_chunk_precise hs c1) as [[h' eqs]|] eqn:?.
     { intros POST__s POST__c HPOST.
       intros δs δc -> hs' hc' ->.
-      unfold approx, ApproxPath.
-      cbv [SMut.put_heap SMut.bind_right T]. cbn. intros Hwp.
-      eapply (approx_assert_formulas Hpc1 eqs) in Hwp; eauto. destruct Hwp as [Heqs HPOST1].
-      cbv [CMut.bind CMut.put_heap CMut.bind_right CMut.assert_formula
-           T CMut.angelic_list CMut.dijkstra].
-      rewrite CDijk.wp_angelic_list.
+      unfold ℛ, RefineProp.
+      cbv [SHeapSpecM.put_heap SHeapSpecM.bind_right T]. cbn. intros Hwp.
+      eapply (refine_assert_formulas Hpc1 eqs) in Hwp; eauto. destruct Hwp as [Heqs HPOST1].
+      cbv [CHeapSpecM.bind CHeapSpecM.put_heap CHeapSpecM.bind_right CHeapSpecM.assert_formula
+           T CHeapSpecM.angelic_list CHeapSpecM.lift_purem].
+      rewrite CPureSpecM.wp_angelic_list.
       destruct c1; cbn in Heqo; try discriminate Heqo; cbn.
       - destruct (𝑯_precise p) as [[ΔI ΔO prec]|]; try discriminate Heqo.
         remember (eq_rect (𝑯_Ty p) (Env (Term w1)) ts (ΔI ▻▻ ΔO) prec) as ts'.
@@ -1786,60 +1901,62 @@ Module Soundness
         rewrite rew_opp_l in HIn. rewrite Heqc1 in HIn.
         rewrite peval_chunk_sound in HIn.
         eexists; split; eauto. clear HIn.
-        hnf. split; auto. now rewrite <- inst_persist.
+        hnf. rewrite CPureSpecM.wp_assert_eq_chunk.
+        split; auto. now rewrite <- inst_persist.
       - destruct (find_chunk_ptsreg_precise_spec r t hs) as [[h'' eqs''] HIn|];
-          inversion Heqo; subst; clear Heqo.
+          inversion Heqo; subst.
         specialize (HIn ι1 Heqs). rewrite Heqc1 in HIn.
         rewrite peval_chunk_sound in HIn.
         eexists; split; eauto. clear HIn.
-        hnf. split; auto. now rewrite <- inst_persist.
+        hnf. rewrite CPureSpecM.wp_assert_eq_chunk.
+        split; auto. now rewrite <- inst_persist.
     }
-    { apply approx_bind.
-      eapply approx_angelic_list; eauto.
+    { apply refine_bind.
+      apply refine_angelic_list; eauto.
       { hnf. unfold inst at 1, inst_heap, inst_list.
         rewrite heap_extractions_map.
         apply List.map_ext. now intros [].
         eauto using inst_is_duplicable.
       }
+      clear Heqo.
       intros w2 ω12 ι2 -> Hpc2.
-      intros [cs' hs'] [cc' hc'].
-      intros Hch'. inversion Hch'; subst; clear Hch'.
-      apply approx_bind_right.
-      - apply approx_assert_formulas; auto.
-        rewrite SMut.inst_match_chunk.
+      intros [cs' hs'] [cc' hc']. intros Hch'.
+      inversion Hch'; subst; clear Hch'.
+      apply refine_bind.
+      - apply refine_assert_eq_chunk; auto. hnf.
         now rewrite inst_persist, peval_chunk_sound, inst_persist.
-      - intros w3 ω23 ι3 -> Hpc3.
-        rewrite <- inst_persist.
-        apply approx_put_heap; auto.
+      - intros w3 ω23 ι3 -> Hpc3 _ _ _.
+        apply refine_put_heap; auto.
+        now rewrite <- inst_persist.
     }
   Qed.
 
-  Lemma approx_consume {Γ Σ0 pc0} (asn : Assertion Σ0) :
+  Lemma refine_consume {Γ Σ0 pc0} (asn : Assertion Σ0) :
     let w0 := @MkWorld Σ0 pc0 in
     forall
       (ι0 : Valuation w0)
       (Hpc0 : instpc (wco w0) ι0),
-      approx ι0 (@SMut.consume Γ w0 asn) (CMut.consume ι0 asn).
+      ℛ ι0 (@SHeapSpecM.consume Γ w0 asn) (CHeapSpecM.consume ι0 asn).
   Proof.
     induction asn; intros w0 * Hpc; cbn - [wctx Val].
-    - now apply approx_box_assert_formula.
+    - now apply refine_box_assert_formula.
     - intros w1 ω01 ι1 -> Hpc1.
       rewrite <- inst_persist.
-      now apply approx_consume_chunk.
+      now apply refine_consume_chunk.
     - intros w1 ω01 ι1 -> Hpc1.
       rewrite <- inst_persist.
-      now apply approx_consume_chunk_angelic.
+      now apply refine_consume_chunk_angelic.
     - intros w1 ω01 ι1 -> Hpc1.
       rewrite <- inst_persist.
-      apply approx_angelic_match_bool; eauto.
+      apply refine_angelic_match_bool; eauto.
     - intros w1 ω01 ι1 -> Hpc1.
       rewrite <- inst_persist.
-      apply approx_angelic_match_enum; auto.
+      apply refine_angelic_match_enum; auto.
       intros EK1 EK2 HEK. hnf in HEK. subst EK2.
       eauto.
     - intros w1 ω01 ι1 -> Hpc1.
       rewrite <- inst_persist.
-      apply approx_angelic_match_sum; auto.
+      apply refine_angelic_match_sum; auto.
       + intros w2 ω12 ι2 -> Hpc2.
         intros t v ->.
         apply IHasn1; cbn - [inst sub_wk1]; wsimpl; auto.
@@ -1848,21 +1965,21 @@ Module Soundness
         apply IHasn2; cbn - [inst sub_wk1]; wsimpl; auto.
     - intros w1 ω01 ι1 -> Hpc1.
       rewrite <- inst_persist.
-      apply approx_angelic_match_list; auto.
-      eapply approx_four; eauto.
+      apply refine_angelic_match_list; auto.
+      eapply refine_four; eauto.
       intros w2 ω12 ι2 -> Hpc2.
       intros thead vhead ->.
       intros ttail vtail ->.
       apply IHasn2; cbn - [inst sub_wk1]; wsimpl; auto.
     - intros w1 ω01 ι1 -> Hpc1.
       rewrite <- inst_persist.
-      apply approx_angelic_match_prod; auto.
+      apply refine_angelic_match_prod; auto.
       intros w2 ω12 ι2 -> Hpc2.
       intros t1 v1 -> t2 v2 ->.
       apply IHasn; cbn - [inst sub_wk1]; wsimpl; auto.
     - intros w1 ω01 ι1 -> Hpc1.
       rewrite <- inst_persist.
-      apply approx_angelic_match_tuple; auto.
+      apply refine_angelic_match_tuple; auto.
       intros w2 ω12 ι2 -> Hpc2.
       intros ts vs ->.
       apply IHasn; cbn - [Sub inst sub_wk1 sub_id sub_cat_left]; wsimpl; auto.
@@ -1879,7 +1996,7 @@ Module Soundness
       now rewrite inst_sub_cat, inst_subst.
     - intros w1 ω01 ι1 -> Hpc1.
       rewrite <- inst_persist.
-      apply approx_angelic_match_record; auto.
+      apply refine_angelic_match_record; auto.
       intros w2 ω12 ι2 -> Hpc2.
       intros ts vs ->.
       apply IHasn; cbn - [Sub inst sub_wk1 sub_id sub_cat_left]; wsimpl; auto.
@@ -1896,7 +2013,7 @@ Module Soundness
       now rewrite inst_sub_cat, inst_subst.
     - intros w1 ω01 ι1 -> Hpc1.
       rewrite <- inst_persist.
-      apply approx_angelic_match_union; auto.
+      apply refine_angelic_match_union; auto.
       intros UK.
       intros w2 ω12 ι2 -> Hpc2.
       intros ts vs ->.
@@ -1913,86 +2030,89 @@ Module Soundness
       }
       now rewrite inst_sub_cat, inst_subst.
     - intros w1 ω01 ι1 -> Hpc1.
-      apply approx_bind_right; eauto.
-      apply IHasn1; eauto.
+      apply refine_bind; eauto.
+      apply IHasn1; auto.
+      intros ? ? ? -> ? _ _ _.
+      apply IHasn2; auto.
+      rewrite ?inst_sub_snoc, ?sub_acc_trans, ?inst_subst, ?inst_sub_wk1; eauto.
     - intros w1 ω01 ι1 -> Hpc1.
-      apply approx_angelic_binary;
+      apply refine_angelic_binary;
         try apply IHasn1; try apply IHasn2;
         cbn - [inst sub_wk1];
         rewrite ?inst_sub_snoc, ?sub_acc_trans, ?inst_subst, ?inst_sub_wk1; eauto.
     - intros w1 ω01 ι1 -> Hpc1.
-      apply approx_bind.
-      apply approx_angelic; auto.
+      apply refine_bind.
+      apply refine_angelic; auto.
       intros w2 ω02 ι2 -> Hpc2. intros t v ->.
       apply IHasn; cbn - [inst sub_wk1];
         rewrite ?inst_sub_snoc, ?sub_acc_trans, ?inst_subst, ?inst_sub_wk1; eauto.
     - intros w1 ω01 ι1 -> Hpc1.
-      apply approx_debug; auto.
-      apply approx_pure; auto.
+      apply refine_debug; auto.
+      apply refine_pure; auto.
   Qed.
 
-  Lemma approx_call_contract {Γ Δ : PCtx} {τ : Ty} (c : SepContract Δ τ) :
+  Lemma refine_call_contract {Γ Δ : PCtx} {τ : Ty} (c : SepContract Δ τ) :
     forall {w0 : World} {ι0 : Valuation w0} (Hpc0 : instpc (wco w0) ι0),
-      approx ι0 (@SMut.call_contract Γ Δ τ c w0) (@CMut.call_contract Γ Δ τ c).
+      ℛ ι0 (@SHeapSpecM.call_contract Γ Δ τ c w0) (@CHeapSpecM.call_contract Γ Δ τ c).
   Proof.
-    destruct c; cbv [SMut.call_contract CMut.call_contract].
+    destruct c; cbv [SHeapSpecM.call_contract CHeapSpecM.call_contract].
     intros w0 ι0 Hpc0.
     intros args__s args__c Hargs.
-    apply approx_bind; auto.
+    apply refine_bind; auto.
     intros w1 ω01 ι1 -> Hpc1.
     intros evars__s evars__c Hevars.
-    apply approx_bind_right.
-    { apply approx_assert_eq_nenv; auto; hnf.
+    apply refine_bind.
+    { apply refine_assert_eq_nenv; auto; hnf.
       now rewrite Hevars, inst_subst.
       now rewrite Hargs, inst_persist.
     }
-    intros w2 ω12 ι2 -> Hpc2.
-    apply approx_bind_right.
-    { apply approx_consume; wsimpl; auto.
+    intros w2 ω12 ι2 -> Hpc2 _ _ _.
+    apply refine_bind.
+    { apply refine_consume; wsimpl; auto.
       constructor.
     }
-    intros w3 ω23 ι3 -> Hpc3.
-    apply approx_bind.
-    { apply approx_demonic; auto. }
+    intros w3 ω23 ι3 -> Hpc3 _ _ _.
+    apply refine_bind.
+    { apply refine_demonic; auto. }
     intros w4 ω34 ι4 -> Hpc4.
     intros res__s res__c Hres.
-    apply approx_bind_right.
-    { apply approx_produce; auto.
+    apply refine_bind.
+    { apply refine_produce; auto.
       constructor.
       cbn - [inst_env sub_snoc].
       rewrite inst_sub_snoc, inst_persist, ?sub_acc_trans, ?inst_subst.
       now rewrite Hevars, Hres.
     }
-    intros w5 ω45 ι5 -> Hpc5.
-    apply approx_pure; auto.
+    intros w5 ω45 ι5 -> Hpc5 _ _ _.
+    apply refine_pure; auto.
     rewrite Hres. rewrite <- inst_persist.
     reflexivity.
   Qed.
 
-  Lemma approx_call_lemma {Γ Δ : PCtx} (lem : Lemma Δ) :
+  Lemma refine_call_lemma {Γ Δ : PCtx} (lem : Lemma Δ) :
     forall {w0 : World} {ι0 : Valuation w0} (Hpc0 : instpc (wco w0) ι0),
-      approx ι0 (@SMut.call_lemma Γ Δ lem w0) (@CMut.call_lemma Γ Δ lem).
+      ℛ ι0 (@SHeapSpecM.call_lemma Γ Δ lem w0) (@CHeapSpecM.call_lemma Γ Δ lem).
   Proof.
-    destruct lem; cbv [SMut.call_lemma CMut.call_lemma].
+    destruct lem; cbv [SHeapSpecM.call_lemma CHeapSpecM.call_lemma].
     intros w0 ι0 Hpc0.
     intros args__s args__c Hargs.
-    apply approx_bind; auto.
+    apply refine_bind; auto.
     intros w1 ω01 ι1 -> Hpc1.
     intros evars__s evars__c Hevars.
-    apply approx_bind_right.
-    apply approx_assert_formulas; auto.
+    apply refine_bind.
+    apply refine_assert_formulas; auto.
     { rewrite inst_formula_eqs_nctx.
       rewrite inst_persist, inst_subst.
       rewrite Hargs, Hevars.
       reflexivity.
     }
-    intros w2 ω12 ι2 -> Hpc2.
-    apply approx_bind_right.
-    { apply approx_consume; wsimpl; auto.
+    intros w2 ω12 ι2 -> Hpc2 _ _ _.
+    apply refine_bind.
+    { apply refine_consume; wsimpl; auto.
       constructor.
     }
-    intros w3 ω23 ι3 -> Hpc3.
-    { apply approx_produce; auto.
+    intros w3 ω23 ι3 -> Hpc3 _ _ _.
+    { apply refine_produce; auto.
       constructor.
       cbn - [inst_env sub_snoc].
       rewrite inst_persist, sub_acc_trans, inst_subst.
@@ -2000,41 +2120,41 @@ Module Soundness
     }
   Qed.
 
-  Definition ExecApprox (sexec : SMut.Exec) (cexec : CMut.Exec) :=
+  Definition ExecRefine (sexec : SHeapSpecM.Exec) (cexec : CHeapSpecM.Exec) :=
     forall Γ τ (s : Stm Γ τ) (w0 : World) (ι0 : Valuation w0) (Hpc0 : instpc (wco w0) ι0),
-    approx ι0 (@sexec Γ τ s w0) (cexec Γ τ s).
+    ℛ ι0 (@sexec Γ τ s w0) (cexec Γ τ s).
 
-  Lemma approx_exec_aux {cfg} srec crec (HYP : ExecApprox srec crec) :
-    ExecApprox (@SMut.exec_aux cfg srec) (@CMut.exec_aux crec).
+  Lemma refine_exec_aux {cfg} srec crec (HYP : ExecRefine srec crec) :
+    ExecRefine (@SHeapSpecM.exec_aux cfg srec) (@CHeapSpecM.exec_aux crec).
   Proof.
-    unfold ExecApprox.
+    unfold ExecRefine.
     induction s; cbn; intros * ?.
-    - apply approx_pure; auto.
-    - now apply approx_eval_exp.
-    - apply approx_bind; auto.
+    - apply refine_pure; auto.
+    - now apply refine_eval_exp.
+    - apply refine_bind; auto.
       intros w1 ω01 ι1 -> Hpc1.
       intros t v Htv.
-      apply approx_pushpop; auto.
-    - apply approx_pushspops; auto.
-      apply approx_lift.
-    - apply approx_bind; auto.
+      apply refine_pushpop; auto.
+    - apply refine_pushspops; auto.
+      apply refine_lift.
+    - apply refine_bind; auto.
       intros w1 ω01 ι1 -> Hpc1.
       intros t v ->.
-      apply approx_bind_right.
-      apply approx_assign; auto.
-      intros w2 ω12 ι2 -> Hpc2.
-      rewrite <- inst_subst.
-      apply approx_pure; auto.
-    - apply approx_bind.
-      apply approx_eval_exps; auto.
+      apply refine_bind.
+      apply refine_assign; auto.
+      intros w2 ω12 ι2 -> Hpc2 _ _ _.
+      apply refine_pure; auto.
+      hnf in H. now rewrite <- inst_persist in H.
+    - apply refine_bind.
+      apply refine_eval_exps; auto.
       intros w1 ω01 ι1 -> Hpc1.
       intros args__s args__c Hargs.
       destruct (CEnv f).
-      + unfold SMut.call_contract_debug.
+      + unfold SHeapSpecM.call_contract_debug.
         destruct (config_debug_function cfg f).
-        apply approx_debug; auto.
-        apply approx_call_contract; auto.
-        apply approx_call_contract; auto.
+        apply refine_debug; auto.
+        apply refine_call_contract; auto.
+        apply refine_call_contract; auto.
       + intros POST__s POST__c HPOST.
         intros δs1 δc1 ->.
         apply HYP; auto.
@@ -2044,266 +2164,222 @@ Module Soundness
         apply HPOST; auto.
         rewrite <- inst_persist.
         reflexivity.
-    - apply approx_bind.
-      apply approx_get_local; auto.
+    - apply refine_bind.
+      apply refine_get_local; auto.
       intros w1 ω01 ι1 -> Hpc1.
       intros δs1 δc1 ->.
-      apply approx_bind_right.
-      apply approx_put_local; auto.
-      apply approx_lift.
-      intros w2 ω12 ι2 -> Hpc2.
-      apply approx_bind; auto.
+      apply refine_bind.
+      apply refine_put_local; auto.
+      apply refine_lift.
+      intros w2 ω12 ι2 -> Hpc2 _ _ _.
+      apply refine_bind; auto.
       intros w3 ω23 ι3 -> Hpc3.
       intros t v ->.
-      apply approx_bind_right.
-      apply approx_put_local; auto.
+      apply refine_bind.
+      apply refine_put_local; auto.
       rewrite persist_subst.
       hnf. rewrite sub_acc_trans, ?inst_subst; auto.
-      intros w4 ω34 ι4 -> Hpc4.
+      intros w4 ω34 ι4 -> Hpc4 _ _ _.
       rewrite <- inst_persist.
-      apply approx_pure; auto.
-    - apply approx_bind.
-      apply approx_eval_exps; auto.
+      apply refine_pure; auto.
+    - apply refine_bind.
+      apply refine_eval_exps; auto.
       intros w1 ω01 ι1 -> Hpc1.
       intros args__s args__c Hargs.
-      apply approx_call_contract; auto.
-    - apply approx_bind_right; auto.
-      apply approx_bind.
-      apply approx_eval_exps; auto.
-      intros w1 ω01 ι1 -> Hpc1.
-      apply approx_call_lemma; auto.
-    - apply approx_bind.
+      apply refine_call_contract; auto.
+    - apply refine_bind.
+      apply refine_eval_exps; auto.
+      intros w1 ω01 ι1 -> Hpc1 δΔ ? ->.
+      apply refine_bind.
+      apply refine_call_lemma; auto.
+      intros w2 ω12 ι2 -> Hpc2 _ _ _; auto.
+    - apply refine_bind.
       intros POST__s POST__c HPOST.
-      apply approx_eval_exp; auto.
+      apply refine_eval_exp; auto.
       intros w1 ω01 ι1 -> Hpc1.
       intros t v Htv.
-      apply approx_demonic_match_bool; auto.
-    - apply approx_bind_right; auto.
-    - apply approx_bind; auto.
+      apply refine_demonic_match_bool; auto.
+    - apply refine_bind; auto.
+      intros ? ? ? -> ? _ _ _; auto.
+    - apply refine_bind; auto.
       intros POST__s POST__c HPOST.
-      apply approx_eval_exp; auto.
+      apply refine_eval_exp; auto.
       intros w1 ω01 ι1 -> Hpc1.
       intros t v ->.
-      apply approx_bind_right.
-      apply approx_assume_formula; auto.
-      intros w2 ω12 ι2 -> Hpc2.
+      apply refine_bind.
+      apply refine_assume_formula; auto.
+      intros w2 ω12 ι2 -> Hpc2 _ _ _.
       now apply IHs.
-    - apply approx_block.
-    - apply approx_bind; auto.
+    - apply refine_block.
+    - apply refine_bind; auto.
       intros POST__s POST__c HPOST.
-      apply approx_eval_exp; auto.
+      apply refine_eval_exp; auto.
       intros w1 ω01 ι1 -> Hpc1.
       intros t v Htv.
-      apply approx_demonic_match_list; auto.
+      apply refine_demonic_match_list; auto.
       intros w2 ω12 ι2 -> Hpc2.
       intros thead vhead ->.
       intros ttail vtail ->.
-      apply approx_pushspops; auto.
-    - apply approx_bind; auto.
+      apply refine_pushspops; auto.
+    - apply refine_bind; auto.
       intros POST__s POST__c HPOST.
-      apply approx_eval_exp; auto.
+      apply refine_eval_exp; auto.
       intros w1 ω01 ι1 -> Hpc1.
       intros t v Htv.
-      apply approx_demonic_match_sum; auto.
+      apply refine_demonic_match_sum; auto.
       + intros w2 ω12 ι2 -> Hpc2.
         intros tl vl ->.
-        apply approx_pushpop; auto.
+        apply refine_pushpop; auto.
       + intros w2 ω12 ι2 -> Hpc2.
         intros tr vr ->.
-        apply approx_pushpop; auto.
-    - apply approx_bind; auto.
+        apply refine_pushpop; auto.
+    - apply refine_bind; auto.
       intros POST__s POST__c HPOST.
-      apply approx_eval_exp; auto.
+      apply refine_eval_exp; auto.
       intros w1 ω01 ι1 -> Hpc1.
       intros t v Htv.
-      apply approx_demonic_match_prod; auto.
+      apply refine_demonic_match_prod; auto.
       intros w2 ω12 ι2 -> Hpc2.
       intros t1 v1 ->.
       intros t2 v2 ->.
-      apply approx_pushspops; auto.
-    - apply approx_bind; auto.
+      apply refine_pushspops; auto.
+    - apply refine_bind; auto.
       intros POST__s POST__c HPOST.
-      apply approx_eval_exp; auto.
+      apply refine_eval_exp; auto.
       intros w1 ω01 ι1 -> Hpc1.
       intros t v Htv.
-      apply approx_demonic_match_enum; auto.
+      apply refine_demonic_match_enum; auto.
       intros EK1 EK2 ->.
       intros w2 ω12 ι2 -> Hpc2; auto.
-    - apply approx_bind; auto.
+    - apply refine_bind; auto.
       intros POST__s POST__c HPOST.
-      apply approx_eval_exp; auto.
+      apply refine_eval_exp; auto.
       intros w1 ω01 ι1 -> Hpc1.
       intros t v Htv.
-      apply approx_demonic_match_tuple; auto.
+      apply refine_demonic_match_tuple; auto.
       intros w2 ω12 ι2 -> Hpc2.
       intros ts vs Htvs.
-      apply approx_pushspops; auto.
-    - apply approx_bind; auto.
+      apply refine_pushspops; auto.
+    - apply refine_bind; auto.
       intros POST__s POST__c HPOST.
-      apply approx_eval_exp; auto.
+      apply refine_eval_exp; auto.
       intros w1 ω01 ι1 -> Hpc1.
       intros t v Htv.
-      apply approx_demonic_match_union; auto.
+      apply refine_demonic_match_union; auto.
       intros UK.
       intros w2 ω12 ι2 -> Hpc2.
       intros ts vs Htvs.
-      apply approx_pushspops; auto.
-    - apply approx_bind; auto.
+      apply refine_pushspops; auto.
+    - apply refine_bind; auto.
       intros POST__s POST__c HPOST.
-      apply approx_eval_exp; auto.
+      apply refine_eval_exp; auto.
       intros w1 ω01 ι1 -> Hpc1.
       intros t v Htv.
-      apply approx_demonic_match_record; auto.
+      apply refine_demonic_match_record; auto.
       intros w2 ω12 ι2 -> Hpc2.
       intros ts vs Htvs.
-      apply approx_pushspops; auto.
-    - apply approx_bind; auto.
+      apply refine_pushspops; auto.
+    - apply refine_bind; auto.
       intros POST__s POST__c HPOST.
-      apply approx_eval_exp; auto.
+      apply refine_eval_exp; auto.
       intros w1 ω01 ι1 -> Hpc1.
       intros t v Htv.
-      apply approx_demonic_match_bvec; auto.
+      apply refine_demonic_match_bvec; auto.
       intros v1 v2 ->.
       intros w2 ω12 ι2 -> Hpc2.
       auto.
-    - apply approx_bind; auto.
-      apply approx_angelic; auto.
-      intros w1 ω01 ι1 -> Hpc1.
-      intros t v ->.
-      apply approx_bind_right; auto.
-      apply approx_consume_chunk; auto.
-      intros w2 ω12 ι2 -> Hpc2.
-      apply approx_bind_right; auto.
-      rewrite <- inst_persist.
-      apply approx_produce_chunk; auto.
-      intros w3 ω23 ι3 -> Hpc3.
-      apply approx_pure; auto. hnf.
+    - apply refine_bind; auto.
+      apply refine_angelic; auto.
+      intros w1 ω01 ι1 -> Hpc1 t v Htv. hnf in Htv; subst.
+      apply refine_bind; auto.
+      apply refine_consume_chunk; auto.
+      intros w2 ω12 ι2 -> Hpc2 _ _ _.
+      apply refine_bind; auto.
+      apply refine_produce_chunk; auto.
+      rewrite <- inst_persist; auto.
+      intros w3 ω23 ι3 -> Hpc3 _ _ _.
+      apply refine_pure; auto. hnf.
       rewrite (persist_trans (A := STerm _)).
       now rewrite <- ?inst_persist.
-    - apply approx_bind; auto.
-      apply approx_angelic; auto.
+    - apply refine_bind; auto.
+      apply refine_angelic; auto.
       intros w1 ω01 ι1 -> Hpc1.
       intros told v ->.
-      apply approx_bind_right; auto.
-      apply approx_consume_chunk; auto.
-      intros w2 ω12 ι2 -> Hpc2.
-      apply approx_bind; auto.
+      apply refine_bind; auto.
+      apply refine_consume_chunk; auto.
+      intros w2 ω12 ι2 -> Hpc2 _ _ _.
+      apply refine_bind; auto.
       intros w3 ω23 ι3 -> Hpc3.
-      intros tnew v ->.
-      apply approx_bind_right; auto.
-      apply approx_produce_chunk; auto.
-      intros w4 ω34 ι4 -> Hpc4.
-      apply approx_pure; auto.
+      intros tnew v Htnew. hnf in Htnew. subst v.
+      apply refine_bind; auto.
+      apply refine_produce_chunk; auto.
+      intros w4 ω34 ι4 -> Hpc4 _ _ _.
+      apply refine_pure; auto.
       now rewrite <- inst_persist.
-    - apply approx_error.
-    - apply approx_debug; auto.
+    - apply refine_error.
+    - apply refine_debug; auto.
   Qed.
 
-  Lemma approx_exec {cfg n} :
-    ExecApprox (@SMut.exec cfg n) (@CMut.exec n).
+  Lemma refine_exec {cfg n} :
+    ExecRefine (@SHeapSpecM.exec cfg n) (@CHeapSpecM.exec n).
   Proof.
     induction n; cbn.
-    - unfold ExecApprox. intros.
+    - unfold ExecRefine. intros.
       intros POST__s POST__c HPOST.
       intros δs1 δc1 Hδ hs1 hc1 Hh.
       hnf. contradiction.
-    - now apply approx_exec_aux.
+    - now apply refine_exec_aux.
   Qed.
 
-  Lemma approx_exec_contract {cfg : Config} n {Γ τ} (c : SepContract Γ τ) (s : Stm Γ τ) :
+  Lemma refine_exec_contract {cfg : Config} n {Γ τ} (c : SepContract Γ τ) (s : Stm Γ τ) :
     let w0 := {| wctx := sep_contract_logic_variables c; wco := nil |} in
     forall (ι0 : Valuation w0),
-      approx (w := w0) ι0 (@SMut.exec_contract cfg n Γ τ c s) (@CMut.exec_contract n Γ τ c s ι0).
+      ℛ (w := w0) ι0 (@SHeapSpecM.exec_contract cfg n Γ τ c s) (@CHeapSpecM.exec_contract n Γ τ c s ι0).
   Proof.
-    unfold SMut.exec_contract, CMut.exec_contract; destruct c as [Σ δ pre result post]; cbn in *.
+    unfold SHeapSpecM.exec_contract, CHeapSpecM.exec_contract; destruct c as [Σ δ pre result post]; cbn in *.
     intros ι0.
-    apply approx_bind_right.
-    apply approx_produce; wsimpl; cbn; auto.
-    intros w1 ω01 ι1 -> Hpc1.
-    apply approx_bind.
-    apply approx_exec; auto.
+    apply refine_bind.
+    apply refine_produce; wsimpl; cbn; auto.
+    intros w1 ω01 ι1 -> Hpc1 _ _ _.
+    apply refine_bind.
+    apply refine_exec; auto.
     intros w2 ω12 ι2 -> Hpc2.
     intros res__s res__c Hres.
-    apply approx_consume; cbn - [inst]; wsimpl; auto.
+    apply refine_consume; cbn - [inst]; wsimpl; auto.
     constructor.
     f_equal; auto.
   Qed.
 
-  Definition safe_demonic_close {Σ : LCtx} :
-    forall p : 𝕊 Σ,
-      safe (demonic_close p) env.nil ->
-      forall ι : Valuation Σ,
-        safe p ι.
+  Lemma refine_demonic_close {w : World} (P : 𝕊 w) (p : Valuation w -> Prop) :
+    (forall (ι : Valuation w), ℛ ι P (p ι)) ->
+    ℛ (w := wnil) env.nil (demonic_close P) (ForallNamed p).
   Proof.
-    induction Σ; cbn [demonic_close] in *.
-    - intros p Hwp ι.
-      destruct (env.nilView ι). apply Hwp.
-    - intros p Hwp ι.
-      destruct b as [x σ], (env.snocView ι).
-      now apply (IHΣ (demonicv (x∷σ) p)).
-  Qed.
-
-  Lemma approx_postprocessing_prune {w : World} (ι : Valuation w) (P : 𝕊 w) (p : Prop) :
-    approx ι P p ->
-    approx ι (Postprocessing.prune P) p.
-  Proof.
-    unfold approx, ApproxPath.
-    now rewrite ?wsafe_safe, ?safe_debug_safe, Postprocessing.prune_sound.
-  Qed.
-
-  Lemma approx_postprocessing_solve_evars {w : World} (ι : Valuation w) (P : 𝕊 w) (p : Prop) :
-    approx ι P p ->
-    approx ι (Postprocessing.solve_evars P) p.
-  Proof.
-    unfold approx, ApproxPath.
-    now rewrite ?wsafe_safe, ?safe_debug_safe, Postprocessing.solve_evars_sound.
-  Qed.
-
-  Lemma approx_postprocessing_solve_uvars {w : World} (ι : Valuation w) (P : 𝕊 w) (p : Prop) :
-    approx ι P p ->
-    approx ι (Postprocessing.solve_uvars P) p.
-  Proof.
-    unfold approx, ApproxPath.
-    rewrite ?wsafe_safe, ?safe_debug_safe.
-    auto using Postprocessing.solve_uvars_sound.
-  Qed.
-
-  Lemma approx_demonic_close {w : World} (P : 𝕊 w) (p : Valuation w -> Prop) :
-    (forall (ι : Valuation w), approx ι P (p ι)) ->
-    approx (w := wnil) env.nil (demonic_close P) (ForallNamed p).
-  Proof.
-    unfold approx, ApproxPath, ForallNamed. intros HYP Hwp.
+    unfold ℛ, RefineProp, ForallNamed. intros HYP Hwp.
     rewrite env.Forall_forall. intros ι.
     apply HYP. revert Hwp. clear.
     rewrite ?wsafe_safe, ?safe_debug_safe.
     intros Hwp. now apply safe_demonic_close.
   Qed.
 
-  Lemma approx_vcgen {Γ τ} (c : SepContract Γ τ) (body : Stm Γ τ) :
-    approx (w := wnil) env.nil (SMut.VcGen c body) (CMut.ValidContract 1 c body).
+  Lemma refine_vcgen {Γ τ} n (c : SepContract Γ τ) (body : Stm Γ τ) :
+    ℛ (w := wnil) env.nil (SHeapSpecM.vcgen default_config n c body) (CHeapSpecM.vcgen n c body).
   Proof.
-    unfold SMut.VcGen.
-    apply approx_postprocessing_prune.
-    apply approx_postprocessing_solve_uvars.
-    apply approx_postprocessing_prune.
-    apply approx_postprocessing_solve_evars.
-    apply approx_postprocessing_prune.
-    unfold SMut.exec_contract_path, CMut.ValidContract.
-    apply (approx_demonic_close
+    unfold SHeapSpecM.vcgen, CHeapSpecM.vcgen.
+    apply (refine_demonic_close
              (w := {| wctx := sep_contract_logic_variables c; wco := nil |})).
     intros ι.
-    apply approx_exec_contract; auto.
+    apply refine_exec_contract; auto.
     now intros w1 ω01 ι1 -> Hpc1.
   Qed.
 
-  Lemma symbolic_execution_soundness {Γ τ} (c : SepContract Γ τ) (body : Stm Γ τ) :
-    SMut.ValidContract c body ->
-    CMut.ValidContract 1 c body.
+  Lemma symbolic_vcgen_soundness {Γ τ} (c : SepContract Γ τ) (body : Stm Γ τ) :
+    Symbolic.ValidContract c body ->
+    Shallow.ValidContract c body.
   Proof.
-    unfold SMut.ValidContract. intros [Hwp].
-    apply approx_vcgen. now rewrite wsafe_safe, safe_debug_safe.
+    unfold Symbolic.ValidContract. intros [Hwp%postprocess_sound].
+    apply refine_vcgen. now rewrite wsafe_safe, safe_debug_safe.
   Qed.
 
-  (* Print Assumptions symbolic_sound. *)
+  (* Print Assumptions symbolic_vcgen_soundness. *)
 
 End Soundness.
